DPE annotated with comments

share/pulse/examples/dice/dpe/DPE.fst
@@ -47,27 +47,27 @@ open Pulse.Lib.MutexToken
 assume
 val run_stt (#a:Type) (#post:a -> slprop) (f:stt a emp post) : a
 
-let sid_hash (s:sid_t) : SZ.t = SZ.uint16_to_sizet s
+let sid_hash (s:sid_t) : SZ.t = SZ.uint16_to_sizet s  //fstar_code
 
 [@@ Rust_const_fn]
 ```pulse
-fn initialize_global_state ()
-  requires emp
-  returns b:(r:gref & mutex (dpe_inv r))
-  ensures emp
+fn initialize_global_state ()  //pulse_spec
+  requires emp  //pulse_spec
+  returns b:(r:gref & mutex (dpe_inv r))  //pulse_spec
+  ensures emp  //pulse_spec
 {
-  let r = ghost_alloc #_ #pcm all_sids_unused;
-  with _v. rewrite (ghost_pcm_pts_to r (G.reveal (G.hide _v))) as
-                   (ghost_pcm_pts_to r _v);
-  fold (dpe_inv r None);
-  let m = new_mutex (dpe_inv r) None;
-  ((| r, m |) <: (r:gref & mutex (dpe_inv r)))
+  let r = ghost_alloc #_ #pcm all_sids_unused;  //pulse_proof
+  with _v. rewrite (ghost_pcm_pts_to r (G.reveal (G.hide _v))) as  //pulse_proof
+                   (ghost_pcm_pts_to r _v);  //pulse_proof
+  fold (dpe_inv r None);  //pulse_proof
+  let m = new_mutex (dpe_inv r) None;  //pulse_code
+  ((| r, m |) <: (r:gref & mutex (dpe_inv r)))  //pulse_code
 }
 ```
 
-let gst : (r:gref & mutex (dpe_inv r)) = run_stt (initialize_global_state ())
+let gst : (r:gref & mutex (dpe_inv r)) = run_stt (initialize_global_state ())  //pulse_code
 
-let trace_ref = dfst gst
+let trace_ref = dfst gst  //pulse_proof
 
 //
 // DPE API implementation
@@ -83,16 +83,16 @@ let trace_ref = dfst gst
 //
 ```pulse
 ghost
-fn gather_ (r:gref)
-  (v0 v1:pcm_t)
-  requires ghost_pcm_pts_to r v0 **
-           ghost_pcm_pts_to r v1
-  returns _:squash (PCM.composable pcm v0 v1)
-  ensures ghost_pcm_pts_to r (PCM.op pcm v0 v1)
+fn gather_ (r:gref)  //pulse_spec
+  (v0 v1:pcm_t)  //pulse_spec
+  requires ghost_pcm_pts_to r v0 **  //pulse_spec
+           ghost_pcm_pts_to r v1  //pulse_spec
+  returns _:squash (PCM.composable pcm v0 v1)  //pulse_spec
+  ensures ghost_pcm_pts_to r (PCM.op pcm v0 v1)  //pulse_spec
 {
-  ghost_gather r v0 v1;
-  with _v. rewrite (ghost_pcm_pts_to r _v) as
-                   (ghost_pcm_pts_to r (PCM.op pcm v0 v1))
+  ghost_gather r v0 v1;  //pulse_proof
+  with _v. rewrite (ghost_pcm_pts_to r _v) as  //pulse_proof
+                   (ghost_pcm_pts_to r (PCM.op pcm v0 v1))  //pulse_proof
 }
 ```
 
@@ -105,17 +105,17 @@ fn gather_ (r:gref)
 // 
 ```pulse
 ghost
-fn gather_v (r:gref)
-  (v0 v1 v:pcm_t)
-  requires ghost_pcm_pts_to r v0 **
-           ghost_pcm_pts_to r v1 **
-           pure (PCM.composable pcm v0 v1 ==> Map.equal (PCM.op pcm v0 v1) v)
-  ensures ghost_pcm_pts_to r v **
-          pure (PCM.composable pcm v0 v1)
+fn gather_v (r:gref)  //pulse_spec
+  (v0 v1 v:pcm_t)  //pulse_spec
+  requires ghost_pcm_pts_to r v0 **  //pulse_spec
+           ghost_pcm_pts_to r v1 **  //pulse_spec
+           pure (PCM.composable pcm v0 v1 ==> Map.equal (PCM.op pcm v0 v1) v)  //pulse_spec
+  ensures ghost_pcm_pts_to r v **  //pulse_spec
+          pure (PCM.composable pcm v0 v1)  //pulse_spec
 {
-  ghost_gather r v0 v1;
-  with _v. rewrite (ghost_pcm_pts_to r _v) as
-                   (ghost_pcm_pts_to r v)
+  ghost_gather r v0 v1;  //pulse_proof
+  with _v. rewrite (ghost_pcm_pts_to r _v) as  //pulse_proof
+                   (ghost_pcm_pts_to r v)  //pulse_proof
 }
 ```
 
@@ -124,210 +124,210 @@ fn gather_v (r:gref)
 //
 ```pulse
 ghost
-fn share_ (r:gref)
-  (v v0 v1:pcm_t)
-  requires ghost_pcm_pts_to r v **
-           pure (PCM.composable pcm v0 v1 /\
-                 Map.equal (PCM.op pcm v0 v1) v)
-  ensures ghost_pcm_pts_to r v0 **
-          ghost_pcm_pts_to r v1
+fn share_ (r:gref)  //pulse_spec
+  (v v0 v1:pcm_t)  //pulse_spec
+  requires ghost_pcm_pts_to r v **  //pulse_spec
+           pure (PCM.composable pcm v0 v1 /\  //pulse_spec
+                 Map.equal (PCM.op pcm v0 v1) v)  //pulse_spec
+  ensures ghost_pcm_pts_to r v0 **  //pulse_spec
+          ghost_pcm_pts_to r v1  //pulse_spec
 {
-  rewrite (ghost_pcm_pts_to r v) as
-          (ghost_pcm_pts_to r (PCM.op pcm v0 v1));
-  ghost_share r v0 v1;
+  rewrite (ghost_pcm_pts_to r v) as  //pulse_proof
+          (ghost_pcm_pts_to r (PCM.op pcm v0 v1));  //pulse_proof
+  ghost_share r v0 v1;  //pulse_proof
 }
 ```
 
 noextract
-let full (t0:trace) = Some #perm 1.0R, t0
+let full (t0:trace) = Some #perm 1.0R, t0  //pulse_proof
 
 noextract
-let half (t0:trace) = Some #perm 0.5R, t0
+let half (t0:trace) = Some #perm 0.5R, t0  //pulse_proof
 
 ```pulse
 ghost
-fn upd_sid_pts_to
-  (r:gref) (sid:sid_t)
-  (#t0 #t1:trace)
-  (s:g_session_state { valid_transition t0 s })
+fn upd_sid_pts_to  //pulse_spec
+  (r:gref) (sid:sid_t)  //pulse_spec
+  (#t0 #t1:trace)  //pulse_spec
+  (s:g_session_state { valid_transition t0 s })  //pulse_spec
 
-  requires sid_pts_to r sid t0 **
-           sid_pts_to r sid t1
-  ensures sid_pts_to r sid (next_trace t0 s) **
-          sid_pts_to r sid (next_trace t0 s) **
+  requires sid_pts_to r sid t0 **  //pulse_spec
+           sid_pts_to r sid t1  //pulse_spec
+  ensures sid_pts_to r sid (next_trace t0 s) **  //pulse_spec
+          sid_pts_to r sid (next_trace t0 s) **  //pulse_spec
           pure (t0 == t1)
 {
-  unfold (sid_pts_to r sid t0);
-  unfold (sid_pts_to r sid t1);
+  unfold (sid_pts_to r sid t0);  //pulse_proof
+  unfold (sid_pts_to r sid t1);  //pulse_proof
 
-  gather_v r (singleton sid 0.5R t0)
-             (singleton sid 0.5R t1)
-             (singleton sid 1.0R t0);
+  gather_v r (singleton sid 0.5R t0)  //pulse_proof
+             (singleton sid 0.5R t1)  //pulse_proof
+             (singleton sid 1.0R t0);  //pulse_proof
 
-  let fp : PCM.frame_preserving_upd trace_pcm (full t0) (full (next_trace t0 s)) =
-    mk_frame_preserving_upd t0 s;
+  let fp : PCM.frame_preserving_upd trace_pcm (full t0) (full (next_trace t0 s)) =  //pulse_proof
+    mk_frame_preserving_upd t0 s;  //pulse_proof
 
-  assert (pure (Map.equal (Map.upd (singleton sid 1.0R t0) sid (full (next_trace t0 s)))
-                          (singleton sid 1.0R (next_trace t0 s))));
+  assert (pure (Map.equal (Map.upd (singleton sid 1.0R t0) sid (full (next_trace t0 s)))  //pulse_proof
+                          (singleton sid 1.0R (next_trace t0 s))));  //pulse_proof
 
-  let fp : PCM.frame_preserving_upd pcm (singleton sid 1.0R t0) (singleton sid 1.0R (next_trace t0 s)) =
-    PM.lift_frame_preserving_upd #_ #_ #trace_pcm
-      (full t0)
-      (full (next_trace t0 s))
-      fp
-      (singleton sid 1.0R t0) sid;
+  let fp : PCM.frame_preserving_upd pcm (singleton sid 1.0R t0) (singleton sid 1.0R (next_trace t0 s)) =  //pulse_proof
+    PM.lift_frame_preserving_upd #_ #_ #trace_pcm  //pulse_proof
+      (full t0)  //pulse_proof
+      (full (next_trace t0 s))  //pulse_proof
+      fp  //pulse_proof
+      (singleton sid 1.0R t0) sid;  //pulse_proof
 
-  ghost_write r
-    (singleton sid 1.0R t0)
-    (singleton sid 1.0R (next_trace t0 s))
-    fp;
+  ghost_write r  //pulse_proof
+    (singleton sid 1.0R t0)  //pulse_proof
+    (singleton sid 1.0R (next_trace t0 s))  //pulse_proof
+    fp;  //pulse_proof
 
-  share_ r (singleton sid 1.0R (next_trace t0 s))
-           (singleton sid 0.5R (next_trace t0 s))
-           (singleton sid 0.5R (next_trace t0 s));
+  share_ r (singleton sid 1.0R (next_trace t0 s))  //pulse_proof
+           (singleton sid 0.5R (next_trace t0 s))  //pulse_proof
+           (singleton sid 0.5R (next_trace t0 s));  //pulse_proof
 
-  fold (sid_pts_to r sid (next_trace t0 s));
-  fold (sid_pts_to r sid (next_trace t0 s));
+  fold (sid_pts_to r sid (next_trace t0 s));  //pulse_proof
+  fold (sid_pts_to r sid (next_trace t0 s));  //pulse_proof
 }
 ```
 
 let safe_incr (i:U16.t)
   : r:option U16.t { Some? r ==> (U16.v (Some?.v r) == U16.v i + 1) } =
 
-  let open FStar.UInt16 in
-  if i <^ 0xffffus
-  then Some (i +^ 1us)
-  else None
+  let open FStar.UInt16 in  //fstar_code
+  if i <^ 0xffffus  //fstar_code
+  then Some (i +^ 1us)  //fstar_code
+  else None  //fstar_code
 
 noextract
-let session_table_eq_on_range
-  (pht0 pht1:pht_t)
-  (i j:nat)
-  : prop =
-  forall (k:sid_t). i <= U16.v k && U16.v k < j ==> PHT.lookup pht0 k == PHT.lookup pht1 k
+let session_table_eq_on_range  //pulse_spec
+  (pht0 pht1:pht_t)  //pulse_spec
+  (i j:nat)  //pulse_spec
+  : prop =  //pulse_spec
+  forall (k:sid_t). i <= U16.v k && U16.v k < j ==> PHT.lookup pht0 k == PHT.lookup pht1 k  //pulse_spec
 
 ```pulse
 ghost
-fn frame_session_perm_at_sid
-  (r:gref)
-  (pht0 pht1:pht_t)
-  (i j:nat)
-  (_:squash (session_table_eq_on_range pht0 pht1 i j))
-  (sid:(sid:nat { i <= sid /\ sid < j }))
-  requires session_perm r pht0 sid
-  ensures session_perm r pht1 sid
+fn frame_session_perm_at_sid  //pulse_spec
+  (r:gref)  //pulse_spec
+  (pht0 pht1:pht_t)  //pulse_spec
+  (i j:nat)  //pulse_spec
+  (_:squash (session_table_eq_on_range pht0 pht1 i j))  //pulse_spec
+  (sid:(sid:nat { i <= sid /\ sid < j }))  //pulse_spec
+  requires session_perm r pht0 sid  //pulse_spec
+  ensures session_perm r pht1 sid  //pulse_spec
 {
-  if (UInt.fits sid 16) {
-    let sid16 = U16.uint_to_t sid;
-    rewrite (session_perm r pht0 sid) as
-            (session_state_perm r pht0 sid16);
-    unfold session_state_perm;
-    fold (session_state_perm r pht1 sid16);
-    rewrite (session_state_perm r pht1 sid16) as
-            (session_perm r pht1 sid)
-  } else {
-    rewrite (session_perm r pht0 sid) as
-            (session_perm r pht1 sid)
+  if (UInt.fits sid 16) {  //pulse_proof
+    let sid16 = U16.uint_to_t sid;  //pulse_proof
+    rewrite (session_perm r pht0 sid) as  //pulse_proof
+            (session_state_perm r pht0 sid16);  //pulse_proof
+    unfold session_state_perm;  //pulse_proof
+    fold (session_state_perm r pht1 sid16);  //pulse_proof
+    rewrite (session_state_perm r pht1 sid16) as  //pulse_proof
+            (session_perm r pht1 sid)  //pulse_proof
+  } else {  //pulse_proof
+    rewrite (session_perm r pht0 sid) as  //pulse_proof
+            (session_perm r pht1 sid)  //pulse_proof
   }
 }
 ```
 
 ```pulse
 ghost
-fn frame_session_perm_on_range
-  (r:gref)
-  (pht0 pht1:pht_t)
-  (i j:nat)
-  requires on_range (session_perm r pht0) i j **
-           pure (session_table_eq_on_range pht0 pht1 i j)
-  ensures on_range (session_perm r pht1) i j
+fn frame_session_perm_on_range  //pulse_spec
+  (r:gref)  //pulse_spec
+  (pht0 pht1:pht_t)  //pulse_spec
+  (i j:nat)  //pulse_spec
+  requires on_range (session_perm r pht0) i j **  //pulse_spec
+           pure (session_table_eq_on_range pht0 pht1 i j)  //pulse_spec
+  ensures on_range (session_perm r pht1) i j  //pulse_spec
 {
-  Pulse.Lib.OnRange.on_range_weaken
-    (session_perm r pht0)
-    (session_perm r pht1)
-    i j
-    (frame_session_perm_at_sid r pht0 pht1 i j ())
+  Pulse.Lib.OnRange.on_range_weaken  //pulse_proof
+    (session_perm r pht0)  //pulse_proof
+    (session_perm r pht1)  //pulse_proof
+    i j  //pulse_proof
+    (frame_session_perm_at_sid r pht0 pht1 i j ())  //pulse_proof
 }
 ```
 
-let emp_to_start_valid () : Lemma (valid_transition emp_trace G_SessionStart) = ()
+let emp_to_start_valid () : Lemma (valid_transition emp_trace G_SessionStart) = ()  //fstar_proof
 
 #push-options "--fuel 0 --ifuel 2 --split_queries no --z3rlimit_factor 2"
 ```pulse
-fn __open_session (s:st)
-  requires dpe_inv trace_ref (Some s)
-  returns b:(st & option sid_t)
-  ensures dpe_inv trace_ref (Some (fst b)) **
-          open_session_client_perm (snd b)
+fn __open_session (s:st)  //pulse_spec
+  requires dpe_inv trace_ref (Some s)  //pulse_spec
+  returns b:(st & option sid_t)  //pulse_spec
+  ensures dpe_inv trace_ref (Some (fst b)) **  //pulse_spec
+          open_session_client_perm (snd b)  //pulse_spec
 {
-  unfold (dpe_inv trace_ref (Some s));
+  unfold (dpe_inv trace_ref (Some s));  //pulse_proof
 
-  let ctr = s.st_ctr;
-  let tbl = s.st_tbl;
+  let ctr = s.st_ctr;  //pulse_code
+  let tbl = s.st_tbl;  //pulse_code
 
-  rewrite each
-    s.st_ctr as ctr,
-    s.st_tbl as tbl;
+  rewrite each  //pulse_proof
+    s.st_ctr as ctr,  //pulse_proof
+    s.st_tbl as tbl;  //pulse_proof
 
-  with pht. assert (models tbl pht);
-  assert (on_range (session_perm trace_ref pht) 0 (U16.v ctr));
-  assert (ghost_pcm_pts_to trace_ref (sids_above_unused ctr));
+  with pht. assert (models tbl pht);  //pulse_proof
+  assert (on_range (session_perm trace_ref pht) 0 (U16.v ctr));  //pulse_proof
+  assert (ghost_pcm_pts_to trace_ref (sids_above_unused ctr));  //pulse_proof
 
-  let copt = safe_incr ctr;
+  let copt = safe_incr ctr;  //pulse_code
 
-  match copt {
-    None -> {
-      let s = { st_ctr = ctr; st_tbl = tbl };
-      let ret = s, None #sid_t;
-      rewrite each
-        ctr as (fst ret).st_ctr,
-        tbl as (fst ret).st_tbl;
-      fold (dpe_inv trace_ref (Some (fst ret)));
-      rewrite emp as (open_session_client_perm (snd ret));
-      ret
+  match copt {  //pulse_code
+    None -> {  //pulse_code
+      let s = { st_ctr = ctr; st_tbl = tbl };  //pulse_code
+      let ret = s, None #sid_t;  //pulse_code
+      rewrite each  //pulse_proof
+        ctr as (fst ret).st_ctr,  //pulse_proof
+        tbl as (fst ret).st_tbl;  //pulse_proof
+      fold (dpe_inv trace_ref (Some (fst ret)));  //pulse_proof
+      rewrite emp as (open_session_client_perm (snd ret));  //pulse_proof
+      ret  //pulse_code
     }
 
-    Some ctr1 -> {
-      let ret = HT.insert_if_not_full tbl ctr SessionStart;
-      let tbl1 = fst ret;
-      let b = snd ret;
-      rewrite each fst ret as tbl1;
-      with pht1. assert (models tbl1 pht1);
-      if b {
-        share_ trace_ref (sids_above_unused ctr)
-                         (sids_above_unused ctr1)
-                         (singleton ctr 1.0R emp_trace);
-        share_ trace_ref (singleton ctr 1.0R emp_trace)
-                         (singleton ctr 0.5R emp_trace)
-                         (singleton ctr 0.5R emp_trace);
-        fold (sid_pts_to trace_ref ctr emp_trace);
-        fold (sid_pts_to trace_ref ctr emp_trace);
-        emp_to_start_valid ();
-        upd_sid_pts_to trace_ref ctr #emp_trace #emp_trace G_SessionStart;
-        rewrite emp as (session_state_related SessionStart G_SessionStart);
-        fold (session_state_perm trace_ref pht1 ctr);
-        rewrite (session_state_perm trace_ref pht1 ctr) as
-                (session_perm trace_ref pht1 (U16.v ctr));
-        frame_session_perm_on_range trace_ref pht pht1 0 (U16.v ctr);
-        on_range_snoc () #(session_perm trace_ref pht1) #0 #(U16.v ctr);
-        let s = { st_ctr = ctr1; st_tbl = tbl1 };
-        let ret = s, Some ctr;
-        rewrite each
-          ctr1 as (fst ret).st_ctr,
-          tbl1 as (fst ret).st_tbl;
-        fold (dpe_inv trace_ref (Some (fst ret)));
-        fold (open_session_client_perm (Some ctr));
-        ret
-      } else {
-        let s = { st_ctr = ctr; st_tbl = tbl1 };
-        let ret = s, None #sid_t;
-        rewrite each
-          tbl1 as (fst ret).st_tbl,
-          pht1 as pht,
-          ctr as (fst ret).st_ctr;
-        fold (dpe_inv trace_ref (Some (fst ret)));
-        rewrite emp as (open_session_client_perm (snd ret));
-        ret
+    Some ctr1 -> {  //pulse_code
+      let ret = HT.insert_if_not_full tbl ctr SessionStart;  //pulse_code
+      let tbl1 = fst ret;  //pulse_code
+      let b = snd ret;  //pulse_code
+      rewrite each fst ret as tbl1;  //pulse_proof
+      with pht1. assert (models tbl1 pht1);  //pulse_proof
+      if b {  //pulse_code
+        share_ trace_ref (sids_above_unused ctr)  //pulse_proof
+                         (sids_above_unused ctr1)  //pulse_proof
+                         (singleton ctr 1.0R emp_trace);  //pulse_proof
+        share_ trace_ref (singleton ctr 1.0R emp_trace)  //pulse_proof
+                         (singleton ctr 0.5R emp_trace)  //pulse_proof
+                         (singleton ctr 0.5R emp_trace);  //pulse_proof
+        fold (sid_pts_to trace_ref ctr emp_trace);  //pulse_proof
+        fold (sid_pts_to trace_ref ctr emp_trace);  //pulse_proof
+        emp_to_start_valid ();  //pulse_proof
+        upd_sid_pts_to trace_ref ctr #emp_trace #emp_trace G_SessionStart;  //pulse_proof
+        rewrite emp as (session_state_related SessionStart G_SessionStart);  //pulse_proof
+        fold (session_state_perm trace_ref pht1 ctr);  //pulse_proof
+        rewrite (session_state_perm trace_ref pht1 ctr) as  //pulse_proof
+                (session_perm trace_ref pht1 (U16.v ctr));  //pulse_proof
+        frame_session_perm_on_range trace_ref pht pht1 0 (U16.v ctr);  //pulse_proof
+        on_range_snoc () #(session_perm trace_ref pht1) #0 #(U16.v ctr);  //pulse_proof
+        let s = { st_ctr = ctr1; st_tbl = tbl1 };  //pulse_code
+        let ret = s, Some ctr;  //pulse_code
+        rewrite each  //pulse_proof
+          ctr1 as (fst ret).st_ctr,  //pulse_proof
+          tbl1 as (fst ret).st_tbl;  //pulse_proof
+        fold (dpe_inv trace_ref (Some (fst ret)));  //pulse_proof
+        fold (open_session_client_perm (Some ctr));  //pulse_proof
+        ret  //pulse_code
+      } else {  //pulse_code
+        let s = { st_ctr = ctr; st_tbl = tbl1 };  //pulse_code
+        let ret = s, None #sid_t;  //pulse_code
+        rewrite each  //pulse_proof
+          tbl1 as (fst ret).st_tbl,  //pulse_proof
+          pht1 as pht,  //pulse_proof
+          ctr as (fst ret).st_ctr;  //pulse_proof
+        fold (dpe_inv trace_ref (Some (fst ret)));  //pulse_proof
+        rewrite emp as (open_session_client_perm (snd ret));  //pulse_proof
+        ret  //pulse_code
       }
     }
   }
@@ -336,36 +336,36 @@ fn __open_session (s:st)
 #pop-options
 
 ```pulse
-fn maybe_mk_session_tbl (sopt:option st)
-  requires dpe_inv trace_ref sopt
-  returns s:st
-  ensures dpe_inv trace_ref (Some s)
+fn maybe_mk_session_tbl (sopt:option st)  //pulse_spec
+  requires dpe_inv trace_ref sopt  //pulse_spec
+  returns s:st  //pulse_spec
+  ensures dpe_inv trace_ref (Some s)  //pulse_spec
 {
-  match sopt {
-    None -> {
-      let tbl = HT.alloc #sid_t #session_state sid_hash 256sz;
-      let s = {
-        st_ctr = 0us;
-        st_tbl = tbl;
+  match sopt {  //pulse_code
+    None -> {  //pulse_code
+      let tbl = HT.alloc #sid_t #session_state sid_hash 256sz;  //pulse_code
+      let s = {  //pulse_code
+        st_ctr = 0us;  //pulse_code
+        st_tbl = tbl;  //pulse_code
       };
 
-      rewrite each tbl as s.st_tbl;
+      rewrite each tbl as s.st_tbl;  //pulse_proof
 
-      unfold dpe_inv;
-      assert (pure (Map.equal all_sids_unused (sids_above_unused s.st_ctr)));
-      rewrite (ghost_pcm_pts_to trace_ref all_sids_unused) as
-              (ghost_pcm_pts_to trace_ref (sids_above_unused s.st_ctr));
+      unfold dpe_inv;  //pulse_proof
+      assert (pure (Map.equal all_sids_unused (sids_above_unused s.st_ctr)));  //pulse_proof
+      rewrite (ghost_pcm_pts_to trace_ref all_sids_unused) as  //pulse_proof
+              (ghost_pcm_pts_to trace_ref (sids_above_unused s.st_ctr));  //pulse_proof
 
-      with pht. assert (models s.st_tbl pht);
-      on_range_empty (session_perm trace_ref pht) 0;
-      rewrite (on_range (session_perm trace_ref pht) 0 0) as
-              (on_range (session_perm trace_ref pht) 0 (U16.v s.st_ctr));
+      with pht. assert (models s.st_tbl pht);  //pulse_proof
+      on_range_empty (session_perm trace_ref pht) 0;  //pulse_proof
+      rewrite (on_range (session_perm trace_ref pht) 0 0) as  //pulse_proof
+              (on_range (session_perm trace_ref pht) 0 (U16.v s.st_ctr));  //pulse_proof
   
-      fold (dpe_inv trace_ref (Some s));
-      s
+      fold (dpe_inv trace_ref (Some s));  //pulse_proof
+      s  //pulse_code
     }
-    Some s -> {
-      s
+    Some s -> {  //pulse_code
+      s  //pulse_code
     }
   }
 }
@@ -373,210 +373,210 @@ fn maybe_mk_session_tbl (sopt:option st)
 
 ```pulse
 ghost
-fn to_dpe_inv_trace_ref (#s:option st) ()
-  requires dpe_inv (Mkdtuple2?._1 gst) s
-  ensures dpe_inv trace_ref s
+fn to_dpe_inv_trace_ref (#s:option st) ()  //pulse_spec
+  requires dpe_inv (Mkdtuple2?._1 gst) s  //pulse_spec
+  ensures dpe_inv trace_ref s  //pulse_spec
 {
-  rewrite (dpe_inv (Mkdtuple2?._1 gst) s) as
-          (dpe_inv trace_ref s)
+  rewrite (dpe_inv (Mkdtuple2?._1 gst) s) as  //pulse_proof
+          (dpe_inv trace_ref s)  //pulse_proof
 }
 ```
 
 ```pulse
 ghost
-fn from_dpe_inv_trace_ref (#s:option st) ()
-  requires dpe_inv trace_ref s
-  ensures dpe_inv (Mkdtuple2?._1 gst) s
+fn from_dpe_inv_trace_ref (#s:option st) ()  //pulse_spec
+  requires dpe_inv trace_ref s  //pulse_spec
+  ensures dpe_inv (Mkdtuple2?._1 gst) s  //pulse_spec
 {
-  rewrite (dpe_inv trace_ref s) as
-          (dpe_inv (Mkdtuple2?._1 gst) s)
+  rewrite (dpe_inv trace_ref s) as  //pulse_proof
+          (dpe_inv (Mkdtuple2?._1 gst) s)  //pulse_proof
 }
 ```
 
 ```pulse
-fn open_session ()
-  requires emp
-  returns r:(option sid_t)
-  ensures open_session_client_perm r
+fn open_session ()  //pulse_spec
+  requires emp  //pulse_spec
+  returns r:(option sid_t)  //pulse_spec
+  ensures open_session_client_perm r  //pulse_spec
 {
-  let mg = M.lock (dsnd gst);
-  to_dpe_inv_trace_ref ();
+  let mg = M.lock (dsnd gst);  //pulse_code
+  to_dpe_inv_trace_ref ();  //pulse_proof
 
-  let sopt = M.replace #(option st) mg None;
+  let sopt = M.replace #(option st) mg None;  //pulse_code
 
-  let s = maybe_mk_session_tbl sopt;
-  let ret = __open_session s;
-  let s = fst ret;
-  let sid_opt = snd ret;
-  rewrite each
-    fst ret as s,
-    snd ret as sid_opt;
-  mg := Some s;
+  let s = maybe_mk_session_tbl sopt;  //pulse_code
+  let ret = __open_session s;  //pulse_code
+  let s = fst ret;  //pulse_code
+  let sid_opt = snd ret;  //pulse_code
+  rewrite each  //pulse_proof
+    fst ret as s,  //pulse_proof
+    snd ret as sid_opt;  //pulse_proof
+  mg := Some s;  //pulse_code
 
-  from_dpe_inv_trace_ref ();
-  M.unlock (dsnd gst) mg;
+  from_dpe_inv_trace_ref ();  //pulse_proof
+  M.unlock (dsnd gst) mg;  //pulse_code
   
-  sid_opt
+  sid_opt  //pulse_code
 }
 ```
 
 [@@allow_ambiguous]
 ```pulse
 ghost
-fn gather_sid_pts_to (sid:sid_t) (#t0 #t1:trace)
-  requires sid_pts_to trace_ref sid t0 **
-           sid_pts_to trace_ref sid t1
-  ensures ghost_pcm_pts_to trace_ref (singleton sid 1.0R t0) **
-          pure (t0 == t1)
+fn gather_sid_pts_to (sid:sid_t) (#t0 #t1:trace)  //pulse_spec
+  requires sid_pts_to trace_ref sid t0 **  //pulse_spec
+           sid_pts_to trace_ref sid t1  //pulse_spec
+  ensures ghost_pcm_pts_to trace_ref (singleton sid 1.0R t0) **  //pulse_spec
+          pure (t0 == t1)  //pulse_spec
 {
-  unfold (sid_pts_to trace_ref sid t0);
-  unfold (sid_pts_to trace_ref sid t1);
-  gather_ trace_ref (singleton sid 0.5R t0) (singleton sid 0.5R t1);
-  with v. assert (ghost_pcm_pts_to trace_ref v);
-  assert (pure (Map.equal v (singleton sid 1.0R t0)));
-  rewrite (ghost_pcm_pts_to trace_ref v) as
-          (ghost_pcm_pts_to trace_ref (singleton sid 1.0R t0))
+  unfold (sid_pts_to trace_ref sid t0);  //pulse_proof
+  unfold (sid_pts_to trace_ref sid t1);  //pulse_proof
+  gather_ trace_ref (singleton sid 0.5R t0) (singleton sid 0.5R t1);  //pulse_proof
+  with v. assert (ghost_pcm_pts_to trace_ref v);  //pulse_proof
+  assert (pure (Map.equal v (singleton sid 1.0R t0)));  //pulse_proof
+  rewrite (ghost_pcm_pts_to trace_ref v) as  //pulse_proof
+          (ghost_pcm_pts_to trace_ref (singleton sid 1.0R t0))  //pulse_proof
 }
 ```
 
 ```pulse
 ghost
-fn share_sid_pts_to (sid:sid_t) (#t:trace)
-  requires ghost_pcm_pts_to trace_ref (singleton sid 1.0R t)
-  ensures sid_pts_to trace_ref sid t **
-          sid_pts_to trace_ref sid t
+fn share_sid_pts_to (sid:sid_t) (#t:trace)  //pulse_spec
+  requires ghost_pcm_pts_to trace_ref (singleton sid 1.0R t)  //pulse_spec
+  ensures sid_pts_to trace_ref sid t **  //pulse_spec
+          sid_pts_to trace_ref sid t  //pulse_spec
 {
-  share_ trace_ref (singleton sid 1.0R t)
-                   (singleton sid 0.5R t)
-                   (singleton sid 0.5R t);
-  fold sid_pts_to;
-  fold sid_pts_to
+  share_ trace_ref (singleton sid 1.0R t)  //pulse_proof
+                   (singleton sid 0.5R t)  //pulse_proof
+                   (singleton sid 0.5R t);  //pulse_proof
+  fold sid_pts_to;  //pulse_proof
+  fold sid_pts_to  //pulse_proof
 }
 ```
 
 ```pulse
 ghost
-fn upd_singleton
-  (sid:sid_t)
-  (#t:trace)
-  (s:g_session_state { valid_transition t s })
-  requires ghost_pcm_pts_to trace_ref (singleton sid 1.0R t)
-  ensures ghost_pcm_pts_to trace_ref (singleton sid 1.0R (next_trace t s))
+fn upd_singleton  //pulse_spec
+  (sid:sid_t)  //pulse_spec
+  (#t:trace)  //pulse_spec
+  (s:g_session_state { valid_transition t s })  //pulse_spec
+  requires ghost_pcm_pts_to trace_ref (singleton sid 1.0R t)  //pulse_spec
+  ensures ghost_pcm_pts_to trace_ref (singleton sid 1.0R (next_trace t s))  //pulse_spec
 {
-  let fp : PCM.frame_preserving_upd trace_pcm (full t) (full (next_trace t s)) =
-    mk_frame_preserving_upd t s;
+  let fp : PCM.frame_preserving_upd trace_pcm (full t) (full (next_trace t s)) =  //pulse_proof
+    mk_frame_preserving_upd t s;  //pulse_proof
 
-  assert (pure (Map.equal (Map.upd (singleton sid 1.0R t) sid (full (next_trace t s)))
-                          (singleton sid 1.0R (next_trace t s))));
+  assert (pure (Map.equal (Map.upd (singleton sid 1.0R t) sid (full (next_trace t s)))  //pulse_proof
+                          (singleton sid 1.0R (next_trace t s))));  //pulse_proof
 
-  let fp : PCM.frame_preserving_upd pcm (singleton sid 1.0R t) (singleton sid 1.0R (next_trace t s)) =
-    PM.lift_frame_preserving_upd #_ #_ #trace_pcm
-      (full t)
-      (full (next_trace t s))
-      fp
-      (singleton sid 1.0R t) sid;
+  let fp : PCM.frame_preserving_upd pcm (singleton sid 1.0R t) (singleton sid 1.0R (next_trace t s)) =  //pulse_proof
+    PM.lift_frame_preserving_upd #_ #_ #trace_pcm  //pulse_proof
+      (full t)  //pulse_proof
+      (full (next_trace t s))  //pulse_proof
+      fp  //pulse_proof
+      (singleton sid 1.0R t) sid;  //pulse_proof
 
-  ghost_write trace_ref
-    (singleton sid 1.0R t)
-    (singleton sid 1.0R (next_trace t s))
-    fp;
+  ghost_write trace_ref  //pulse_proof
+    (singleton sid 1.0R t)  //pulse_proof
+    (singleton sid 1.0R (next_trace t s))  //pulse_proof
+    fp;  //pulse_proof
 }
 ```
 
 #push-options "--fuel 0 --ifuel 2 --split_queries no --z3rlimit_factor 2"
 ```pulse
-fn replace_session
-  (sid:sid_t)
-  (t:G.erased trace)
-  (sst:session_state)
-  (gsst:g_session_state { valid_transition t gsst})
+fn replace_session  //pulse_spec
+  (sid:sid_t)  //pulse_spec
+  (t:G.erased trace)  //pulse_spec
+  (sst:session_state)  //pulse_spec
+  (gsst:g_session_state { valid_transition t gsst})  //pulse_spec
 
-  requires sid_pts_to trace_ref sid t **
-           session_state_related sst gsst
+  requires sid_pts_to trace_ref sid t **  //pulse_spec
+           session_state_related sst gsst  //pulse_spec
 
-  returns r:session_state
+  returns r:session_state  //pulse_spec
 
-  ensures session_state_related r (current_state t) **
-          sid_pts_to trace_ref sid (next_trace t gsst)
+  ensures session_state_related r (current_state t) **  //pulse_spec
+          sid_pts_to trace_ref sid (next_trace t gsst)  //pulse_spec
 {
-  let mg = M.lock (dsnd gst);
-  to_dpe_inv_trace_ref ();
+  let mg = M.lock (dsnd gst);  //pulse_code
+  to_dpe_inv_trace_ref ();  //pulse_proof
 
-  let sopt = M.replace mg None;
-  match sopt {
-    None -> {
-      unfold (dpe_inv trace_ref None);
-      unfold sid_pts_to;
-      gather_ trace_ref all_sids_unused (singleton sid 0.5R t);
-      unreachable ()
+  let sopt = M.replace mg None;  //pulse_code
+  match sopt {  //pulse_code
+    None -> {  //pulse_code
+      unfold (dpe_inv trace_ref None);  //pulse_proof
+      unfold sid_pts_to;  //pulse_proof
+      gather_ trace_ref all_sids_unused (singleton sid 0.5R t);  //pulse_proof
+      unreachable ()  //pulse_proof
     }
-    Some s -> {
-      unfold (dpe_inv trace_ref (Some s));
-      let ctr = s.st_ctr;
-      let tbl = s.st_tbl;
-      rewrite each
-        s.st_ctr as ctr,
-        s.st_tbl as tbl;
-      with pht0. assert (models tbl pht0);
-      assert (on_range (session_perm trace_ref pht0) 0 (U16.v ctr));
-      if U16.lt sid ctr {
-        on_range_get (U16.v sid) #(session_perm trace_ref pht0) #0 #(U16.v ctr);
-        rewrite (session_perm trace_ref pht0 (U16.v sid)) as
-                (session_state_perm trace_ref pht0 sid);
-        unfold session_state_perm;
-        gather_sid_pts_to sid;
-        with t1. assert (ghost_pcm_pts_to trace_ref (singleton sid 1.0R t1));
-        assert (pure (t1 == t));
-        let ret = HT.lookup tbl sid;
-        let tbl = tfst ret;
-        let b = tsnd ret;
-        let idx = tthd ret;
-        rewrite each
-          tfst ret as tbl,
-          tsnd ret as b,
-          tthd ret as idx;
-        with pht. assert (models tbl pht);
-        if b {
-          match idx {
-            Some idx -> {
-              let ret = HT.replace #_ #_ #pht tbl idx sid sst ();
-              let tbl = fst ret;
-              let st = snd ret;
-              rewrite each
-                fst ret as tbl,
-                snd ret as st;
-              assert (session_state_related sst gsst);
-              with sst' gsst'. assert (
-                session_state_related sst' gsst' **
-                session_state_related sst gsst
+    Some s -> {  //pulse_code
+      unfold (dpe_inv trace_ref (Some s));  //pulse_proof
+      let ctr = s.st_ctr;  //pulse_code
+      let tbl = s.st_tbl;  //pulse_code
+      rewrite each  //pulse_proof
+        s.st_ctr as ctr,  //pulse_proof
+        s.st_tbl as tbl;  //pulse_proof
+      with pht0. assert (models tbl pht0);  //pulse_proof
+      assert (on_range (session_perm trace_ref pht0) 0 (U16.v ctr));  //pulse_proof
+      if U16.lt sid ctr {  //pulse_code
+        on_range_get (U16.v sid) #(session_perm trace_ref pht0) #0 #(U16.v ctr);  //pulse_proof
+        rewrite (session_perm trace_ref pht0 (U16.v sid)) as  //pulse_proof
+                (session_state_perm trace_ref pht0 sid);  //pulse_proof
+        unfold session_state_perm;  //pulse_proof
+        gather_sid_pts_to sid;  //pulse_proof
+        with t1. assert (ghost_pcm_pts_to trace_ref (singleton sid 1.0R t1));  //pulse_proof
+        assert (pure (t1 == t));  //pulse_proof
+        let ret = HT.lookup tbl sid;  //pulse_code
+        let tbl = tfst ret;  //pulse_code
+        let b = tsnd ret;  //pulse_code
+        let idx = tthd ret;  //pulse_code
+        rewrite each  //pulse_proof
+          tfst ret as tbl,  //pulse_proof
+          tsnd ret as b,  //pulse_proof
+          tthd ret as idx;  //pulse_proof
+        with pht. assert (models tbl pht);  //pulse_proof
+        if b {  //pulse_code
+          match idx {  //pulse_code
+            Some idx -> {  //pulse_code
+              let ret = HT.replace #_ #_ #pht tbl idx sid sst ();  //pulse_code
+              let tbl = fst ret;  //pulse_code
+              let st = snd ret;  //pulse_code
+              rewrite each  //pulse_proof
+                fst ret as tbl,  //pulse_proof
+                snd ret as st;  //pulse_proof
+              assert (session_state_related sst gsst);  //pulse_proof
+              with sst' gsst'. assert (  //pulse_proof
+                session_state_related sst' gsst' **  //pulse_proof
+                session_state_related sst gsst  //pulse_proof
               );
-              rewrite (session_state_related sst' gsst')
-                   as (session_state_related st (current_state t1));
-              with pht. assert (models tbl pht);
-              upd_singleton sid #t1 gsst;
-              share_sid_pts_to sid;
-              rewrite (session_state_related sst gsst) as
-                      (session_state_related sst (current_state (next_trace t1 gsst)));
-              fold (session_state_perm trace_ref pht sid);
-              rewrite (session_state_perm trace_ref pht sid) as
-                      (session_perm trace_ref pht (U16.v sid));
-              frame_session_perm_on_range trace_ref pht0 pht 0 (U16.v sid);
-              frame_session_perm_on_range trace_ref pht0 pht (U16.v sid + 1) (U16.v ctr);
-              on_range_put 0 (U16.v sid) (U16.v ctr) #(session_perm trace_ref pht);
-              let s = { st_ctr = ctr; st_tbl = tbl };
-              rewrite each
-                ctr as s.st_ctr,
-                tbl as s.st_tbl;
-              fold (dpe_inv trace_ref (Some s));
-              mg := Some s;
+              rewrite (session_state_related sst' gsst')  //pulse_proof
+                   as (session_state_related st (current_state t1));  //pulse_proof
+              with pht. assert (models tbl pht);  //pulse_proof
+              upd_singleton sid #t1 gsst;  //pulse_proof
+              share_sid_pts_to sid;  //pulse_proof
+              rewrite (session_state_related sst gsst) as  //pulse_proof
+                      (session_state_related sst (current_state (next_trace t1 gsst)));  //pulse_proof
+              fold (session_state_perm trace_ref pht sid);  //pulse_proof
+              rewrite (session_state_perm trace_ref pht sid) as  //pulse_proof
+                      (session_perm trace_ref pht (U16.v sid));  //pulse_proof
+              frame_session_perm_on_range trace_ref pht0 pht 0 (U16.v sid);  //pulse_proof
+              frame_session_perm_on_range trace_ref pht0 pht (U16.v sid + 1) (U16.v ctr);  //pulse_proof
+              on_range_put 0 (U16.v sid) (U16.v ctr) #(session_perm trace_ref pht);  //pulse_proof
+              let s = { st_ctr = ctr; st_tbl = tbl };  //pulse_code
+              rewrite each  //pulse_proof
+                ctr as s.st_ctr,  //pulse_proof
+                tbl as s.st_tbl;  //pulse_proof
+              fold (dpe_inv trace_ref (Some s));  //pulse_proof
+              mg := Some s;  //pulse_code
 
-              from_dpe_inv_trace_ref ();
-              M.unlock (dsnd gst) mg;
+              from_dpe_inv_trace_ref ();  //pulse_proof
+              M.unlock (dsnd gst) mg;  //pulse_code
               
-              st
+              st  //pulse_code
             }
-            None -> {
-              unreachable ()
+            None -> {  //pulse_code
+              unreachable ()  //pulse_proof
             }
           }
         } else {
@@ -587,9 +587,9 @@ fn replace_session
           unreachable ()
         }
       } else {
-        unfold sid_pts_to;
-        gather_ trace_ref (sids_above_unused ctr) (singleton sid 0.5R t);
-        unreachable ()
+        unfold sid_pts_to;  //pulse_proof
+        gather_ trace_ref (sids_above_unused ctr) (singleton sid 0.5R t);  //pulse_proof
+        unreachable ()  //pulse_proof
       }
     }
   }
@@ -598,111 +598,111 @@ fn replace_session
 #pop-options
 
 ```pulse
-fn init_engine_ctxt
-  (uds:A.array U8.t { A.length uds == SZ.v uds_len })
-  (#p:perm)
-  (#uds_bytes:Ghost.erased (Seq.seq U8.t))
-  requires A.pts_to uds #p uds_bytes
-  returns ctxt:context_t
-  ensures A.pts_to uds #p uds_bytes **
-          context_perm ctxt (Engine_context_repr uds_bytes)
+fn init_engine_ctxt  //pulse_spec
+  (uds:A.array U8.t { A.length uds == SZ.v uds_len })  //pulse_spec
+  (#p:perm)  //pulse_spec
+  (#uds_bytes:Ghost.erased (Seq.seq U8.t))  //pulse_spec
+  requires A.pts_to uds #p uds_bytes  //pulse_spec
+  returns ctxt:context_t  //pulse_spec
+  ensures A.pts_to uds #p uds_bytes **  //pulse_spec
+          context_perm ctxt (Engine_context_repr uds_bytes)  //pulse_spec
 { 
-  let uds_buf = V.alloc 0uy uds_len;
-  A.pts_to_len uds;
-  V.pts_to_len uds_buf;
+  let uds_buf = V.alloc 0uy uds_len;  //pulse_code
+  A.pts_to_len uds;  //pulse_proof
+  V.pts_to_len uds_buf;  //pulse_proof
 
-  V.to_array_pts_to uds_buf;
-  A.memcpy uds_len uds (V.vec_to_array uds_buf);
-  V.to_vec_pts_to uds_buf;
+  V.to_array_pts_to uds_buf;  //pulse_proof
+  A.memcpy uds_len uds (V.vec_to_array uds_buf);  //pulse_code
+  V.to_vec_pts_to uds_buf;  //pulse_proof
 
-  let engine_context = mk_engine_context_t uds_buf;
+  let engine_context = mk_engine_context_t uds_buf;  //pulse_code
 
-  rewrite each uds_buf as (engine_context.uds);
-  fold (engine_context_perm engine_context uds_bytes);
+  rewrite each uds_buf as (engine_context.uds);  //pulse_proof
+  fold (engine_context_perm engine_context uds_bytes);  //pulse_proof
 
-  let ctxt = mk_context_t_engine engine_context;
-  rewrite (engine_context_perm engine_context uds_bytes) 
-       as (context_perm ctxt (Engine_context_repr uds_bytes));
-  ctxt
+  let ctxt = mk_context_t_engine engine_context;  //pulse_code
+  rewrite (engine_context_perm engine_context uds_bytes)   //pulse_proof
+       as (context_perm ctxt (Engine_context_repr uds_bytes));  //pulse_proof
+  ctxt  //pulse_code
 }
 ```
 
-let session_state_tag_related (s:session_state) (gs:g_session_state) : GTot bool =
-  match s, gs with
-  | SessionStart, G_SessionStart
-  | InUse, G_InUse _
-  | SessionClosed, G_SessionClosed _
-  | SessionError, G_SessionError _
-  | Available _, G_Available _ -> true
-  | _ -> false
+let session_state_tag_related (s:session_state) (gs:g_session_state) : GTot bool =  //pulse_spec
+  match s, gs with  //pulse_spec
+  | SessionStart, G_SessionStart  //pulse_spec
+  | InUse, G_InUse _  //pulse_spec
+  | SessionClosed, G_SessionClosed _  //pulse_spec
+  | SessionError, G_SessionError _  //pulse_spec
+  | Available _, G_Available _ -> true  //pulse_spec
+  | _ -> false  //pulse_spec
 
 
 ```pulse
 ghost
-fn intro_session_state_tag_related (s:session_state) (gs:g_session_state)
-  requires session_state_related s gs
-  ensures session_state_related s gs **
-          pure (session_state_tag_related s gs)
+fn intro_session_state_tag_related (s:session_state) (gs:g_session_state)  //pulse_spec
+  requires session_state_related s gs  //pulse_spec
+  ensures session_state_related s gs **  //pulse_spec
+          pure (session_state_tag_related s gs)  //pulse_spec
 {
-  let b = session_state_tag_related s gs;
-  if b {
-    ()
-  } else {
-    rewrite (session_state_related s gs) as
-            (pure False);
-    unreachable ()
+  let b = session_state_tag_related s gs;  //pulse_proof
+  if b {  //pulse_proof
+    ()  //pulse_proof
+  } else {  //pulse_proof
+    rewrite (session_state_related s gs) as  //pulse_proof
+            (pure False);  //pulse_proof
+    unreachable ()  //pulse_proof
   }
 }
 ```
 
 #push-options "--fuel 2 --ifuel 2 --split_queries no"
 ```pulse
-fn initialize_context (sid:sid_t) 
-  (t:G.erased trace { trace_valid_for_initialize_context t })
-  (#p:perm) (#uds_bytes:Ghost.erased (Seq.seq U8.t))
-  (uds:A.larray U8.t (SZ.v uds_len)) 
+fn initialize_context (sid:sid_t)  //pulse_spec
+  (t:G.erased trace { trace_valid_for_initialize_context t })  //pulse_spec
+  (#p:perm) (#uds_bytes:Ghost.erased (Seq.seq U8.t))  //pulse_spec
+  (uds:A.larray U8.t (SZ.v uds_len))   //pulse_spec
                        
-  requires A.pts_to uds #p uds_bytes **
-           sid_pts_to trace_ref sid t
+  requires A.pts_to uds #p uds_bytes **  //pulse_spec
+           sid_pts_to trace_ref sid t  //pulse_spec
 
-  ensures A.pts_to uds #p uds_bytes **
-          initialize_context_client_perm sid uds_bytes
+  ensures A.pts_to uds #p uds_bytes **  //pulse_spec
+          initialize_context_client_perm sid uds_bytes  //pulse_spec
 {
-  rewrite emp as (session_state_related InUse (G_InUse (current_state t)));
-  let s = replace_session sid t InUse (G_InUse (current_state t));
-  with t1. assert (sid_pts_to trace_ref sid t1);
+  rewrite emp as (session_state_related InUse (G_InUse (current_state t)));  //pulse_proof
+  let s = replace_session sid t InUse (G_InUse (current_state t));  //pulse_code
+  with t1. assert (sid_pts_to trace_ref sid t1);  //pulse_proof
 
-  match s {
-    SessionStart -> {
-      rewrite (session_state_related s (current_state t)) as emp;
-      let context = init_engine_ctxt uds;
-      let s = Available { context };
-      rewrite (context_perm context (Engine_context_repr uds_bytes)) as
-              (session_state_related s (G_Available (Engine_context_repr uds_bytes)));
-      let s = replace_session sid t1 s (G_Available (Engine_context_repr uds_bytes));
-      intro_session_state_tag_related s (current_state t1);
-      with _x _y. rewrite (session_state_related _x _y) as emp;
-      fold (initialize_context_client_perm sid uds_bytes)
+  match s {  //pulse_code
+    SessionStart -> {  //pulse_code
+      rewrite (session_state_related s (current_state t)) as emp;  //pulse_proof
+      let context = init_engine_ctxt uds;  //pulse_code
+      let s = Available { context };  //pulse_code
+      rewrite (context_perm context (Engine_context_repr uds_bytes)) as  //pulse_proof
+              (session_state_related s (G_Available (Engine_context_repr uds_bytes)));  //pulse_proof
+      let s = replace_session sid t1 s (G_Available (Engine_context_repr uds_bytes));  //pulse_code
+      intro_session_state_tag_related s (current_state t1);  //pulse_proof
+      with _x _y. rewrite (session_state_related _x _y) as emp;  //pulse_proof
+      fold (initialize_context_client_perm sid uds_bytes)  //pulse_proof
     }
-    InUse -> {
-      rewrite (session_state_related s (current_state t)) as
-              (pure False);
-      unreachable ()
+    InUse -> {  //pulse_code
+      rewrite (session_state_related s (current_state t)) as  //pulse_proof
+              (pure False);  //pulse_proof
+      unreachable ()  //pulse_proof
     }
-    SessionClosed -> {
-      rewrite (session_state_related s (current_state t)) as
-              (pure False);
-      unreachable ()
+    SessionClosed -> {  //pulse_code
+      rewrite (session_state_related s (current_state t)) as  //pulse_proof
+              (pure False);  //pulse_proof
+      unreachable ()  //pulse_proof
     }
-    SessionError -> {
-      rewrite (session_state_related s (current_state t)) as
-              (pure False);
-      unreachable ()
+    SessionError -> {  //pulse_code
+      rewrite (session_state_related s (current_state t)) as  //pulse_proof
+              (pure False);  //pulse_proof
+      unreachable ()  //pulse_proof
     }
-    Available _ -> {
-      rewrite (session_state_related s (current_state t)) as
-              (pure False);
-      unreachable ()
+    Available _ -> {  //pulse_code
+      rewrite (session_state_related s (current_state t)) as  //pulse_proof
+              (pure False);  //pulse_proof
+      unreachable ()  //pulse_proof
     }
   }
 }
@@ -710,370 +710,370 @@ fn initialize_context (sid:sid_t)
 #pop-options
 
 ```pulse
-fn init_l0_ctxt
-  (cdi:A.array U8.t { A.length cdi == SZ.v dice_digest_len })
-  (#engine_repr:erased engine_record_repr)
-  (#s:erased (Seq.seq U8.t))
-  (#uds_bytes:erased (Seq.seq U8.t))
-  (_:squash (cdi_functional_correctness s uds_bytes engine_repr /\
-             l0_is_authentic engine_repr))
-  requires A.pts_to cdi s
-  returns ctxt:l0_context_t
-  ensures
-    A.pts_to cdi s **
-    l0_context_perm ctxt (mk_l0_context_repr_t uds_bytes s engine_repr)
+fn init_l0_ctxt  //pulse_spec
+  (cdi:A.array U8.t { A.length cdi == SZ.v dice_digest_len })  //pulse_spec
+  (#engine_repr:erased engine_record_repr)  //pulse_spec
+  (#s:erased (Seq.seq U8.t))  //pulse_spec
+  (#uds_bytes:erased (Seq.seq U8.t))  //pulse_spec
+  (_:squash (cdi_functional_correctness s uds_bytes engine_repr /\  //pulse_spec
+             l0_is_authentic engine_repr))  //pulse_spec
+  requires A.pts_to cdi s  //pulse_spec
+  returns ctxt:l0_context_t  //pulse_spec
+  ensures  //pulse_spec
+    A.pts_to cdi s **  //pulse_spec
+    l0_context_perm ctxt (mk_l0_context_repr_t uds_bytes s engine_repr)  //pulse_spec
 {
-  let cdi_buf = V.alloc 0uy dice_digest_len;
-  A.pts_to_len cdi;
-  V.pts_to_len cdi_buf;
+  let cdi_buf = V.alloc 0uy dice_digest_len;  //pulse_code
+  A.pts_to_len cdi;  //pulse_proof
+  V.pts_to_len cdi_buf;  //pulse_proof
 
-  V.to_array_pts_to cdi_buf;
-  A.memcpy dice_digest_len cdi (V.vec_to_array cdi_buf);
-  V.to_vec_pts_to cdi_buf;
+  V.to_array_pts_to cdi_buf;  //pulse_proof
+  A.memcpy dice_digest_len cdi (V.vec_to_array cdi_buf);  //pulse_code
+  V.to_vec_pts_to cdi_buf;  //pulse_proof
   
-  let l0_context = mk_l0_context_t cdi_buf;
-  let l0_context_repr = hide (mk_l0_context_repr_t uds_bytes s engine_repr);
-  rewrite each cdi_buf as (l0_context.cdi);
-  fold (l0_context_perm l0_context l0_context_repr);
-  l0_context
+  let l0_context = mk_l0_context_t cdi_buf;  //pulse_code
+  let l0_context_repr = hide (mk_l0_context_repr_t uds_bytes s engine_repr);  //pulse_proof
+  rewrite each cdi_buf as (l0_context.cdi);  //pulse_proof
+  fold (l0_context_perm l0_context l0_context_repr);  //pulse_proof
+  l0_context  //pulse_code
 }
 ```
 
 ```pulse
-fn init_l1_ctxt
-  (cdi:erased (Seq.seq U8.t))
-  (deviceID_label_len:(n:erased U32.t { valid_hkdf_lbl_len n }))
-  (aliasKey_label_len:(n:erased U32.t { valid_hkdf_lbl_len n }))
-  (deviceIDCSR_ingredients:erased deviceIDCSR_ingredients_t)
-  (aliasKeyCRT_ingredients:erased aliasKeyCRT_ingredients_t)
-  (deviceID_pub:V.lvec U8.t 32)
-  (aliasKey_priv:V.lvec U8.t 32)
-  (aliasKey_pub:V.lvec U8.t 32)
-  (deviceIDCSR_len:(n:U32.t { valid_deviceIDCSR_ingredients deviceIDCSR_ingredients n }))
-  (deviceIDCSR:V.lvec U8.t (U32.v deviceIDCSR_len))
-  (aliasKeyCRT_len:(n:U32.t { valid_aliasKeyCRT_ingredients aliasKeyCRT_ingredients n }))
-  (aliasKeyCRT:V.lvec U8.t (U32.v aliasKeyCRT_len))
-  (repr:erased l0_record_repr_t)
-  (#deviceID_pub_repr #aliasKey_pub_repr #aliasKey_priv_repr
-   #deviceIDCSR_repr #aliasKeyCRT_repr:erased (Seq.seq U8.t))
-  (_:squash (l0_post
-     cdi
-     repr.fwid
-     deviceID_label_len
-     repr.deviceID_label
-     aliasKey_label_len
-     repr.aliasKey_label
-     deviceIDCSR_ingredients
-     aliasKeyCRT_ingredients
-     deviceID_pub_repr
-     aliasKey_pub_repr
-     aliasKey_priv_repr
-     deviceIDCSR_len
-     deviceIDCSR_repr
-     aliasKeyCRT_len
-     aliasKeyCRT_repr))
-  requires V.pts_to deviceID_pub deviceID_pub_repr ** 
-           V.pts_to aliasKey_pub aliasKey_pub_repr ** 
-           V.pts_to aliasKey_priv aliasKey_priv_repr ** 
-           V.pts_to deviceIDCSR deviceIDCSR_repr **
-           V.pts_to aliasKeyCRT aliasKeyCRT_repr **
-           pure (V.is_full_vec deviceID_pub /\
-                 V.is_full_vec aliasKey_pub /\
-                 V.is_full_vec aliasKey_priv /\
-                 V.is_full_vec deviceIDCSR /\
-                  V.is_full_vec aliasKeyCRT)
-  returns ctxt:l1_context_t
-  ensures 
-    l1_context_perm ctxt (mk_l1_context_repr_t
-      cdi deviceID_label_len aliasKey_label_len deviceIDCSR_ingredients aliasKeyCRT_ingredients
-      deviceID_pub_repr aliasKey_pub_repr aliasKey_priv_repr
-      deviceIDCSR_len deviceIDCSR_repr aliasKeyCRT_len aliasKeyCRT_repr repr)
+fn init_l1_ctxt  //pulse_spec
+  (cdi:erased (Seq.seq U8.t))  //pulse_spec
+  (deviceID_label_len:(n:erased U32.t { valid_hkdf_lbl_len n }))  //pulse_spec
+  (aliasKey_label_len:(n:erased U32.t { valid_hkdf_lbl_len n }))  //pulse_spec
+  (deviceIDCSR_ingredients:erased deviceIDCSR_ingredients_t)  //pulse_spec
+  (aliasKeyCRT_ingredients:erased aliasKeyCRT_ingredients_t)  //pulse_spec
+  (deviceID_pub:V.lvec U8.t 32)  //pulse_spec
+  (aliasKey_priv:V.lvec U8.t 32)  //pulse_spec
+  (aliasKey_pub:V.lvec U8.t 32)  //pulse_spec
+  (deviceIDCSR_len:(n:U32.t { valid_deviceIDCSR_ingredients deviceIDCSR_ingredients n }))  //pulse_spec
+  (deviceIDCSR:V.lvec U8.t (U32.v deviceIDCSR_len))  //pulse_spec
+  (aliasKeyCRT_len:(n:U32.t { valid_aliasKeyCRT_ingredients aliasKeyCRT_ingredients n }))  //pulse_spec
+  (aliasKeyCRT:V.lvec U8.t (U32.v aliasKeyCRT_len))  //pulse_spec
+  (repr:erased l0_record_repr_t)  //pulse_spec
+  (#deviceID_pub_repr #aliasKey_pub_repr #aliasKey_priv_repr  //pulse_spec
+   #deviceIDCSR_repr #aliasKeyCRT_repr:erased (Seq.seq U8.t))  //pulse_spec
+  (_:squash (l0_post  //pulse_spec
+     cdi  //pulse_spec
+     repr.fwid  //pulse_spec
+     deviceID_label_len  //pulse_spec
+     repr.deviceID_label  //pulse_spec
+     aliasKey_label_len  //pulse_spec
+     repr.aliasKey_label  //pulse_spec
+     deviceIDCSR_ingredients  //pulse_spec
+     aliasKeyCRT_ingredients  //pulse_spec
+     deviceID_pub_repr  //pulse_spec
+     aliasKey_pub_repr  //pulse_spec
+     aliasKey_priv_repr  //pulse_spec
+     deviceIDCSR_len  //pulse_spec
+     deviceIDCSR_repr  //pulse_spec
+     aliasKeyCRT_len  //pulse_spec
+     aliasKeyCRT_repr))  //pulse_spec
+  requires V.pts_to deviceID_pub deviceID_pub_repr **  //pulse_spec
+           V.pts_to aliasKey_pub aliasKey_pub_repr **  //pulse_spec
+           V.pts_to aliasKey_priv aliasKey_priv_repr **  //pulse_spec
+           V.pts_to deviceIDCSR deviceIDCSR_repr **  //pulse_spec
+           V.pts_to aliasKeyCRT aliasKeyCRT_repr **  //pulse_spec
+           pure (V.is_full_vec deviceID_pub /\  //pulse_spec
+                 V.is_full_vec aliasKey_pub /\  //pulse_spec
+                 V.is_full_vec aliasKey_priv /\  //pulse_spec
+                 V.is_full_vec deviceIDCSR /\  //pulse_spec
+                  V.is_full_vec aliasKeyCRT)  //pulse_spec
+  returns ctxt:l1_context_t  //pulse_spec
+  ensures  //pulse_spec
+    l1_context_perm ctxt (mk_l1_context_repr_t  //pulse_spec
+      cdi deviceID_label_len aliasKey_label_len deviceIDCSR_ingredients aliasKeyCRT_ingredients  //pulse_spec
+      deviceID_pub_repr aliasKey_pub_repr aliasKey_priv_repr  //pulse_spec
+      deviceIDCSR_len deviceIDCSR_repr aliasKeyCRT_len aliasKeyCRT_repr repr)  //pulse_spec
 {
-  let ctxt = mk_l1_context_t
-    deviceID_pub aliasKey_pub aliasKey_priv deviceIDCSR_len deviceIDCSR aliasKeyCRT_len aliasKeyCRT;
+  let ctxt = mk_l1_context_t  //pulse_code
+    deviceID_pub aliasKey_pub aliasKey_priv deviceIDCSR_len deviceIDCSR aliasKeyCRT_len aliasKeyCRT;  //pulse_code
   
-  let l1_ctxt_repr = hide (mk_l1_context_repr_t
-    cdi deviceID_label_len aliasKey_label_len
-    deviceIDCSR_ingredients aliasKeyCRT_ingredients
-    deviceID_pub_repr aliasKey_pub_repr aliasKey_priv_repr
-    deviceIDCSR_len deviceIDCSR_repr aliasKeyCRT_len aliasKeyCRT_repr
-    repr);
+  let l1_ctxt_repr = hide (mk_l1_context_repr_t  //pulse_proof
+    cdi deviceID_label_len aliasKey_label_len  //pulse_proof
+    deviceIDCSR_ingredients aliasKeyCRT_ingredients  //pulse_proof
+    deviceID_pub_repr aliasKey_pub_repr aliasKey_priv_repr  //pulse_proof
+    deviceIDCSR_len deviceIDCSR_repr aliasKeyCRT_len aliasKeyCRT_repr  //pulse_proof
+    repr);  //pulse_proof
 
-  rewrite each
-    deviceID_pub as ctxt.deviceID_pub,
-    aliasKey_pub as ctxt.aliasKey_pub,
-    aliasKey_priv as ctxt.aliasKey_priv,
-    deviceIDCSR as ctxt.deviceIDCSR,
-    aliasKeyCRT as ctxt.aliasKeyCRT;
+  rewrite each  //pulse_proof
+    deviceID_pub as ctxt.deviceID_pub,  //pulse_proof
+    aliasKey_pub as ctxt.aliasKey_pub,  //pulse_proof
+    aliasKey_priv as ctxt.aliasKey_priv,  //pulse_proof
+    deviceIDCSR as ctxt.deviceIDCSR,  //pulse_proof
+    aliasKeyCRT as ctxt.aliasKeyCRT;  //pulse_proof
 
-  rewrite each
-    cdi as l1_ctxt_repr.cdi,
-    deviceID_pub_repr as l1_ctxt_repr.deviceID_pub,
-    aliasKey_pub_repr as l1_ctxt_repr.aliasKey_pub,
-    aliasKey_priv_repr as l1_ctxt_repr.aliasKey_priv,
-    deviceIDCSR_repr as l1_ctxt_repr.deviceIDCSR,
-    aliasKeyCRT_repr as l1_ctxt_repr.aliasKeyCRT;
+  rewrite each  //pulse_proof
+    cdi as l1_ctxt_repr.cdi,  //pulse_proof
+    deviceID_pub_repr as l1_ctxt_repr.deviceID_pub,  //pulse_proof
+    aliasKey_pub_repr as l1_ctxt_repr.aliasKey_pub,  //pulse_proof
+    aliasKey_priv_repr as l1_ctxt_repr.aliasKey_priv,  //pulse_proof
+    deviceIDCSR_repr as l1_ctxt_repr.deviceIDCSR,  //pulse_proof
+    aliasKeyCRT_repr as l1_ctxt_repr.aliasKeyCRT;  //pulse_proof
 
-  fold (l1_context_perm ctxt l1_ctxt_repr);
-  ctxt
+  fold (l1_context_perm ctxt l1_ctxt_repr);  //pulse_proof
+  ctxt  //pulse_code
 }
 ```
 
 ```pulse
 ghost
-fn l0_record_perm_aux (r1 r2:l0_record_t) (#p:perm) (#repr:l0_record_repr_t)
-  requires l0_record_perm r1 p repr **
-           pure (r1.fwid == r2.fwid /\
-                 r1.deviceID_label_len == r2.deviceID_label_len /\
-                 r1.deviceID_label == r2.deviceID_label /\
-                 r1.aliasKey_label_len == r2.aliasKey_label_len /\
-                 r1.aliasKey_label == r2.aliasKey_label)
-  ensures l0_record_perm r2 p repr
+fn l0_record_perm_aux (r1 r2:l0_record_t) (#p:perm) (#repr:l0_record_repr_t)  //pulse_spec
+  requires l0_record_perm r1 p repr **  //pulse_spec
+           pure (r1.fwid == r2.fwid /\  //pulse_spec
+                 r1.deviceID_label_len == r2.deviceID_label_len /\  //pulse_spec
+                 r1.deviceID_label == r2.deviceID_label /\  //pulse_spec
+                 r1.aliasKey_label_len == r2.aliasKey_label_len /\  //pulse_spec
+                 r1.aliasKey_label == r2.aliasKey_label)  //pulse_spec
+  ensures l0_record_perm r2 p repr  //pulse_spec
 {
-  unfold (l0_record_perm r1 p repr);
-  rewrite (V.pts_to r1.fwid #p repr.fwid) as (V.pts_to r2.fwid #p repr.fwid);
-  rewrite (V.pts_to r1.deviceID_label #p repr.deviceID_label)
-       as (V.pts_to r2.deviceID_label #p repr.deviceID_label);
-  rewrite (V.pts_to r1.aliasKey_label #p repr.aliasKey_label)
-       as (V.pts_to r2.aliasKey_label #p repr.aliasKey_label);
-  fold (l0_record_perm r2 p repr)
+  unfold (l0_record_perm r1 p repr);  //pulse_proof
+  rewrite (V.pts_to r1.fwid #p repr.fwid) as (V.pts_to r2.fwid #p repr.fwid);  //pulse_proof
+  rewrite (V.pts_to r1.deviceID_label #p repr.deviceID_label)  //pulse_proof
+       as (V.pts_to r2.deviceID_label #p repr.deviceID_label);  //pulse_proof
+  rewrite (V.pts_to r1.aliasKey_label #p repr.aliasKey_label)  //pulse_proof
+       as (V.pts_to r2.aliasKey_label #p repr.aliasKey_label);  //pulse_proof
+  fold (l0_record_perm r2 p repr)  //pulse_proof
 }
 ```
 
 noextract
-let context_derives_from_input (r:context_repr_t) (rrepr:repr_t) : prop =
-  match r, rrepr with
-  | L0_context_repr l0_repr, Engine_repr erepr ->
-    l0_repr.repr == erepr
-  | L1_context_repr l1_repr, L0_repr lrepr ->
-    l1_repr.repr == lrepr
-  | _ -> False    
+let context_derives_from_input (r:context_repr_t) (rrepr:repr_t) : prop =  //pulse_spec
+  match r, rrepr with  //pulse_spec
+  | L0_context_repr l0_repr, Engine_repr erepr ->  //pulse_spec
+    l0_repr.repr == erepr  //pulse_spec
+  | L1_context_repr l1_repr, L0_repr lrepr ->  //pulse_spec
+    l1_repr.repr == lrepr  //pulse_spec
+  | _ -> False  //pulse_spec
     
-let maybe_context_perm (r:context_repr_t) (rrepr:repr_t) (c:option context_t) =
-  match c with
-  | Some c ->
-    exists* repr. context_perm c repr **
-                  pure (next_repr r repr /\ context_derives_from_input repr rrepr)
-  | None -> emp
+let maybe_context_perm (r:context_repr_t) (rrepr:repr_t) (c:option context_t) =  //pulse_spec
+  match c with  //pulse_spec
+  | Some c ->  //pulse_spec
+    exists* repr. context_perm c repr **  //pulse_spec
+                  pure (next_repr r repr /\ context_derives_from_input repr rrepr)  //pulse_spec
+  | None -> emp  //pulse_spec
 
 noextract
-let valid_context_and_record_for_derive_child (c:context_repr_t) (r:repr_t) : prop =
-  match c, r with
-  | Engine_context_repr _, Engine_repr _ -> True
-  | L0_context_repr _, L0_repr _ -> True
-  | _ -> False
+let valid_context_and_record_for_derive_child (c:context_repr_t) (r:repr_t) : prop =  //pulse_spec
+  match c, r with  //pulse_spec
+  | Engine_context_repr _, Engine_repr _ -> True  //pulse_spec
+  | L0_context_repr _, L0_repr _ -> True  //pulse_spec
+  | _ -> False  //pulse_spec
 
 ```pulse 
-fn destroy_ctxt (ctxt:context_t) (#repr:erased context_repr_t)
-  requires context_perm ctxt repr
-  ensures emp
+fn destroy_ctxt (ctxt:context_t) (#repr:erased context_repr_t)  //pulse_spec
+  requires context_perm ctxt repr  //pulse_spec
+  ensures emp  //pulse_spec
 {
-  match ctxt
+  match ctxt  //pulse_code
   {
-    Engine_context c ->
+    Engine_context c ->  //pulse_code
     {
-      let uds = rewrite_context_perm_engine c;
-      unfold (engine_context_perm c uds);
-      V.free c.uds;
+      let uds = rewrite_context_perm_engine c;  //pulse_proof
+      unfold (engine_context_perm c uds);  //pulse_proof
+      V.free c.uds;  //pulse_code
     }
-    L0_context c ->
+    L0_context c ->  //pulse_code
     {
-      let r = rewrite_context_perm_l0 c;
-      unfold (l0_context_perm c r);
-      V.free c.cdi;
+      let r = rewrite_context_perm_l0 c;  //pulse_proof
+      unfold (l0_context_perm c r);  //pulse_proof
+      V.free c.cdi;  //pulse_code
     }
-    L1_context c ->
+    L1_context c ->  //pulse_code
     {
-      let r = rewrite_context_perm_l1 c;
-      unfold (l1_context_perm c r);
-      V.free c.deviceID_pub;
-      V.free c.aliasKey_priv;
-      V.free c.aliasKey_pub;
-      V.free c.aliasKeyCRT;
-      V.free c.deviceIDCSR;
+      let r = rewrite_context_perm_l1 c;  //pulse_proof
+      unfold (l1_context_perm c r);  //pulse_proof
+      V.free c.deviceID_pub;  //pulse_code
+      V.free c.aliasKey_priv;  //pulse_code
+      V.free c.aliasKey_pub;  //pulse_code
+      V.free c.aliasKeyCRT;  //pulse_code
+      V.free c.deviceIDCSR;  //pulse_code
     }
   }
 }
 ```
 
 ```pulse
-fn derive_child_from_context
-    (context:context_t)
-    (record:record_t)
-    (#record_repr: erased repr_t)
-    (#context_repr:erased (context_repr_t))
-    (_:squash (valid_context_and_record_for_derive_child context_repr record_repr))
+fn derive_child_from_context  //pulse_spec
+    (context:context_t)  //pulse_spec
+    (record:record_t)  //pulse_spec
+    (#record_repr: erased repr_t)  //pulse_spec
+    (#context_repr:erased (context_repr_t))  //pulse_spec
+    (_:squash (valid_context_and_record_for_derive_child context_repr record_repr))  //pulse_spec
 
-  requires
-    context_perm context context_repr **
-    record_perm record 1.0R record_repr
-  returns res:(option context_t)
-  ensures
-    maybe_context_perm context_repr record_repr res
+  requires  //pulse_spec
+    context_perm context context_repr **  //pulse_spec
+    record_perm record 1.0R record_repr  //pulse_spec
+  returns res:(option context_t)  //pulse_spec
+  ensures  //pulse_spec
+    maybe_context_perm context_repr record_repr res  //pulse_spec
 {
-  intro_context_and_repr_tag_related context context_repr;
-  intro_record_and_repr_tag_related record 1.0R record_repr;
+  intro_context_and_repr_tag_related context context_repr;  //pulse_proof
+  intro_record_and_repr_tag_related record 1.0R record_repr;  //pulse_proof
  
-  match context {
-    Engine_context c -> {
-      match record {
-        Engine_record r -> {
-          let uds_bytes = rewrite_context_perm_engine c;
-          unfold (engine_context_perm c uds_bytes);
+  match context {  //pulse_code
+    Engine_context c -> {  //pulse_code
+      match record {  //pulse_code
+        Engine_record r -> {  //pulse_code
+          let uds_bytes = rewrite_context_perm_engine c;  //pulse_proof
+          unfold (engine_context_perm c uds_bytes);  //pulse_proof
 
-          let engine_record_repr = rewrite_record_perm_engine r;
+          let engine_record_repr = rewrite_record_perm_engine r;  //pulse_proof
 
-          let mut cdi = [| 0uy; dice_digest_len |];
+          let mut cdi = [| 0uy; dice_digest_len |];  //pulse_code
 
-          V.to_array_pts_to c.uds;
-          let ret = EngineCore.engine_main cdi (V.vec_to_array c.uds) r;
-          V.to_vec_pts_to c.uds;
+          V.to_array_pts_to c.uds;  //pulse_proof
+          let ret = EngineCore.engine_main cdi (V.vec_to_array c.uds) r;  //pulse_code
+          V.to_vec_pts_to c.uds;  //pulse_proof
 
-          let r = fst ret;
-          rewrite each fst ret as r;
+          let r = fst ret;  //pulse_code
+          rewrite each fst ret as r;  //pulse_proof
 
-          with s. assert (A.pts_to cdi s);
-          fold (engine_context_perm c uds_bytes);
-          rewrite (engine_context_perm c uds_bytes)
-               as (context_perm (Engine_context c) context_repr);
-          rewrite (engine_record_perm r 1.0R engine_record_repr)
-               as (record_perm (Engine_record r) 1.0R record_repr);
+          with s. assert (A.pts_to cdi s);  //pulse_proof
+          fold (engine_context_perm c uds_bytes);  //pulse_proof
+          rewrite (engine_context_perm c uds_bytes)  //pulse_proof
+               as (context_perm (Engine_context c) context_repr);  //pulse_proof
+          rewrite (engine_record_perm r 1.0R engine_record_repr)  //pulse_proof
+               as (record_perm (Engine_record r) 1.0R record_repr);  //pulse_proof
 
-          destroy_ctxt (Engine_context c);
+          destroy_ctxt (Engine_context c);  //pulse_code
           //
           // TODO: FIXME: deallocate
           //
-          drop_ (record_perm (Engine_record r) 1.0R record_repr);
+          drop_ (record_perm (Engine_record r) 1.0R record_repr);  //pulse_proof
          
-          match snd ret {
-            DICE_SUCCESS -> {
-              let l0_ctxt = init_l0_ctxt cdi #engine_record_repr #s #uds_bytes ();
-              with l0_ctxt_repr. assert (l0_context_perm l0_ctxt l0_ctxt_repr);
-              fold (context_perm (L0_context l0_ctxt) (L0_context_repr l0_ctxt_repr));
-              fold (maybe_context_perm context_repr record_repr (Some (L0_context l0_ctxt)));
-              let ret = Some (L0_context l0_ctxt);
-              rewrite each
-                Some (L0_context l0_ctxt) as ret;
-              ret
+          match snd ret {  //pulse_code
+            DICE_SUCCESS -> {  //pulse_code
+              let l0_ctxt = init_l0_ctxt cdi #engine_record_repr #s #uds_bytes ();  //pulse_code
+              with l0_ctxt_repr. assert (l0_context_perm l0_ctxt l0_ctxt_repr);  //pulse_proof
+              fold (context_perm (L0_context l0_ctxt) (L0_context_repr l0_ctxt_repr));  //pulse_proof
+              fold (maybe_context_perm context_repr record_repr (Some (L0_context l0_ctxt)));  //pulse_proof
+              let ret = Some (L0_context l0_ctxt);  //pulse_code
+              rewrite each  //pulse_proof
+                Some (L0_context l0_ctxt) as ret;  //pulse_proof
+              ret  //pulse_code
             }
 
-            DICE_ERROR -> {
-              A.zeroize dice_digest_len cdi;
-              let ret = None #context_t;
-              rewrite emp as (maybe_context_perm context_repr record_repr ret);
-              ret
+            DICE_ERROR -> {  //pulse_code
+              A.zeroize dice_digest_len cdi;  //pulse_code
+              let ret = None #context_t;  //pulse_code
+              rewrite emp as (maybe_context_perm context_repr record_repr ret);  //pulse_proof
+              ret  //pulse_code
             }
           }
         }
-        L0_record _ -> {
-          unreachable ()
+        L0_record _ -> {  //pulse_code
+          unreachable ()  //pulse_proof
         }
       }
     }
     
-    L0_context c -> {
-      match record {
-        L0_record r -> {
-          let cr = rewrite_context_perm_l0 c;
-          unfold (l0_context_perm c cr);
-          with s. assert (V.pts_to c.cdi s);
+    L0_context c -> {  //pulse_code
+      match record {  //pulse_code
+        L0_record r -> {  //pulse_code
+          let cr = rewrite_context_perm_l0 c;  //pulse_proof
+          unfold (l0_context_perm c cr);  //pulse_proof
+          with s. assert (V.pts_to c.cdi s);  //pulse_proof
 
-          let r0 = rewrite_record_perm_l0 r;
-          unfold (l0_record_perm r 1.0R r0);
+          let r0 = rewrite_record_perm_l0 r;  //pulse_proof
+          unfold (l0_record_perm r 1.0R r0);  //pulse_proof
 
-          let deviceID_pub = V.alloc 0uy (SZ.uint_to_t 32);
-          let aliasKey_pub = V.alloc 0uy (SZ.uint_to_t 32);
-          let aliasKey_priv = V.alloc 0uy (SZ.uint_to_t 32);
-          assume_ (pure (SZ.fits_u32));
-          let deviceIDCSR_len = L0Types.len_of_deviceIDCSR r.deviceIDCSR_ingredients;
-          let aliasKeyCRT_len = L0Types.len_of_aliasKeyCRT r.aliasKeyCRT_ingredients;
-          let deviceIDCSR = V.alloc 0uy (SZ.uint32_to_sizet deviceIDCSR_len);
-          let aliasKeyCRT = V.alloc 0uy (SZ.uint32_to_sizet aliasKeyCRT_len);
+          let deviceID_pub = V.alloc 0uy (SZ.uint_to_t 32);  //pulse_code
+          let aliasKey_pub = V.alloc 0uy (SZ.uint_to_t 32);  //pulse_code
+          let aliasKey_priv = V.alloc 0uy (SZ.uint_to_t 32);  //pulse_code
+          assume_ (pure (SZ.fits_u32));  //pulse_proof
+          let deviceIDCSR_len = L0Types.len_of_deviceIDCSR r.deviceIDCSR_ingredients;  //pulse_code
+          let aliasKeyCRT_len = L0Types.len_of_aliasKeyCRT r.aliasKeyCRT_ingredients;  //pulse_code
+          let deviceIDCSR = V.alloc 0uy (SZ.uint32_to_sizet deviceIDCSR_len);  //pulse_code
+          let aliasKeyCRT = V.alloc 0uy (SZ.uint32_to_sizet aliasKeyCRT_len);  //pulse_code
 
-          V.to_array_pts_to c.cdi;
-          V.to_array_pts_to r.fwid;
-          V.to_array_pts_to r.deviceID_label;
-          V.to_array_pts_to r.aliasKey_label;
-          V.to_array_pts_to deviceID_pub;
-          V.to_array_pts_to aliasKey_pub;
-          V.to_array_pts_to aliasKey_priv;
-          V.to_array_pts_to deviceIDCSR;
-          V.to_array_pts_to aliasKeyCRT;
+          V.to_array_pts_to c.cdi;  //pulse_proof
+          V.to_array_pts_to r.fwid;  //pulse_proof
+          V.to_array_pts_to r.deviceID_label;  //pulse_proof
+          V.to_array_pts_to r.aliasKey_label;  //pulse_proof
+          V.to_array_pts_to deviceID_pub;  //pulse_proof
+          V.to_array_pts_to aliasKey_pub;  //pulse_proof
+          V.to_array_pts_to aliasKey_priv;  //pulse_proof
+          V.to_array_pts_to deviceIDCSR;  //pulse_proof
+          V.to_array_pts_to aliasKeyCRT;  //pulse_proof
 
-          assume_ (pure (A.length (V.vec_to_array c.cdi) == 32));
+          assume_ (pure (A.length (V.vec_to_array c.cdi) == 32));  //pulse_proof
 
-          let _ : unit = l0
-            (V.vec_to_array c.cdi)
-            (V.vec_to_array r.fwid)
-            r.deviceID_label_len
-            (V.vec_to_array r.deviceID_label)
-            r.aliasKey_label_len
-            (V.vec_to_array r.aliasKey_label)
-            r.deviceIDCSR_ingredients
-            r.aliasKeyCRT_ingredients
-            (V.vec_to_array deviceID_pub)
-            (V.vec_to_array aliasKey_pub)
-            (V.vec_to_array aliasKey_priv)
-            deviceIDCSR_len
-            (V.vec_to_array deviceIDCSR)
-            aliasKeyCRT_len
-            (V.vec_to_array aliasKeyCRT);
+          let _ : unit = l0  //pulse_code
+            (V.vec_to_array c.cdi)  //pulse_code
+            (V.vec_to_array r.fwid)  //pulse_code
+            r.deviceID_label_len  //pulse_code
+            (V.vec_to_array r.deviceID_label)  //pulse_code
+            r.aliasKey_label_len  //pulse_code
+            (V.vec_to_array r.aliasKey_label)  //pulse_code
+            r.deviceIDCSR_ingredients  //pulse_code
+            r.aliasKeyCRT_ingredients  //pulse_code
+            (V.vec_to_array deviceID_pub)  //pulse_code
+            (V.vec_to_array aliasKey_pub)  //pulse_code
+            (V.vec_to_array aliasKey_priv)  //pulse_code
+            deviceIDCSR_len  //pulse_code
+            (V.vec_to_array deviceIDCSR)  //pulse_code
+            aliasKeyCRT_len  //pulse_code
+            (V.vec_to_array aliasKeyCRT);  //pulse_code
           
-          V.to_vec_pts_to c.cdi;
-          V.to_vec_pts_to r.fwid;
-          V.to_vec_pts_to r.deviceID_label;
-          V.to_vec_pts_to r.aliasKey_label;
-          V.to_vec_pts_to deviceID_pub;
-          V.to_vec_pts_to aliasKey_pub;
-          V.to_vec_pts_to aliasKey_priv;
-          V.to_vec_pts_to deviceIDCSR;
-          V.to_vec_pts_to aliasKeyCRT;
+          V.to_vec_pts_to c.cdi;  //pulse_proof
+          V.to_vec_pts_to r.fwid;  //pulse_proof
+          V.to_vec_pts_to r.deviceID_label;  //pulse_proof
+          V.to_vec_pts_to r.aliasKey_label;  //pulse_proof
+          V.to_vec_pts_to deviceID_pub;  //pulse_proof
+          V.to_vec_pts_to aliasKey_pub;  //pulse_proof
+          V.to_vec_pts_to aliasKey_priv;  //pulse_proof
+          V.to_vec_pts_to deviceIDCSR;  //pulse_proof
+          V.to_vec_pts_to aliasKeyCRT;  //pulse_proof
 
-          let l1_context : l1_context_t = init_l1_ctxt
-            s
-            (hide r.deviceID_label_len)
-            (hide r.aliasKey_label_len)
-            (hide r.deviceIDCSR_ingredients)
-            (hide r.aliasKeyCRT_ingredients)
-            deviceID_pub
-            aliasKey_priv
-            aliasKey_pub
-            deviceIDCSR_len
-            deviceIDCSR
-            aliasKeyCRT_len
-            aliasKeyCRT
-            r0
-            (magic ());
+          let l1_context : l1_context_t = init_l1_ctxt  //pulse_code
+            s  //pulse_code
+            (hide r.deviceID_label_len)  //pulse_proof
+            (hide r.aliasKey_label_len)  //pulse_proof
+            (hide r.deviceIDCSR_ingredients)  //pulse_proof
+            (hide r.aliasKeyCRT_ingredients)  //pulse_proof
+            deviceID_pub  //pulse_code
+            aliasKey_priv  //pulse_code
+            aliasKey_pub  //pulse_code
+            deviceIDCSR_len  //pulse_code
+            deviceIDCSR  //pulse_code
+            aliasKeyCRT_len  //pulse_code
+            aliasKeyCRT  //pulse_code
+            r0  //pulse_proof
+            (magic ());  //pulse_proof
 
-          fold (l0_context_perm c cr);
-          rewrite (l0_context_perm c cr) as
-                  (context_perm (L0_context c) context_repr);
-          fold (l0_record_perm r 1.0R r0);
-          rewrite (l0_record_perm r 1.0R r0) as
-                  (record_perm (L0_record r) 1.0R record_repr);
+          fold (l0_context_perm c cr);  //pulse_proof
+          rewrite (l0_context_perm c cr) as  //pulse_proof
+                  (context_perm (L0_context c) context_repr);  //pulse_proof
+          fold (l0_record_perm r 1.0R r0);  //pulse_proof
+          rewrite (l0_record_perm r 1.0R r0) as  //pulse_proof
+                  (record_perm (L0_record r) 1.0R record_repr);  //pulse_proof
 
-          destroy_ctxt (L0_context c);
-          drop_ (record_perm (L0_record r) 1.0R record_repr);
+          destroy_ctxt (L0_context c);  //pulse_code
+          drop_ (record_perm (L0_record r) 1.0R record_repr);  //pulse_proof
                     
-          with l1_context_repr. assert (l1_context_perm l1_context l1_context_repr);
+          with l1_context_repr. assert (l1_context_perm l1_context l1_context_repr);  //pulse_proof
           
-          fold (context_perm (L1_context l1_context) (L1_context_repr l1_context_repr));
+          fold (context_perm (L1_context l1_context) (L1_context_repr l1_context_repr));  //pulse_proof
 
-          fold (maybe_context_perm context_repr record_repr (Some (L1_context l1_context)));
-          let ret = Some (L1_context l1_context);
-          rewrite each
-            Some (L1_context l1_context) as ret;
+          fold (maybe_context_perm context_repr record_repr (Some (L1_context l1_context)));  //pulse_proof
+          let ret = Some (L1_context l1_context);  //pulse_code
+          rewrite each  //pulse_proof
+            Some (L1_context l1_context) as ret;  //pulse_proof
 
-          ret
+          ret  //pulse_code
         }
-        Engine_record _ -> {
-          unreachable ()
+        Engine_record _ -> {  //pulse_code
+          unreachable ()  //pulse_proof
         }
       }
     }
 
-    L1_context _ -> {
-      unreachable ()
+    L1_context _ -> {  //pulse_code
+      unreachable ()  //pulse_proof
     }
   }
 }
@@ -1081,225 +1081,225 @@ fn derive_child_from_context
 
 ```pulse
 ghost
-fn rewrite_session_state_related_available
-  context
-  (s:session_state { s == Available { context } })
-  (t:trace)
-  requires session_state_related s (current_state t)
-  returns r:G.erased context_repr_t
-  ensures context_perm context r ** pure (current_state t == G_Available r)
+fn rewrite_session_state_related_available  //pulse_spec
+  context  //pulse_spec
+  (s:session_state { s == Available { context } })  //pulse_spec
+  (t:trace)  //pulse_spec
+  requires session_state_related s (current_state t)  //pulse_spec
+  returns r:G.erased context_repr_t  //pulse_spec
+  ensures context_perm context r ** pure (current_state t == G_Available r)  //pulse_spec
 {
-  let cur = current_state t;
-  intro_session_state_tag_related s cur;
-  let repr = G_Available?.repr cur;
-  rewrite (session_state_related s cur) as
-          (context_perm context repr);
-  hide repr
+  let cur = current_state t;  //pulse_proof
+  intro_session_state_tag_related s cur;  //pulse_proof
+  let repr = G_Available?.repr cur;  //pulse_proof
+  rewrite (session_state_related s cur) as  //pulse_proof
+          (context_perm context repr);  //pulse_proof
+  hide repr  //pulse_proof
 }
 ```
 
 #push-options "--fuel 2 --ifuel 2 --split_queries no"
 ```pulse
-fn derive_child (sid:sid_t)
-  (t:G.erased trace)
-  (record:record_t)
-  (#rrepr:erased repr_t { trace_and_record_valid_for_derive_child t rrepr })
-  requires record_perm record 1.0R rrepr **
-           sid_pts_to trace_ref sid t
-  returns b:bool
-  ensures derive_child_client_perm sid t rrepr b
+fn derive_child (sid:sid_t)  //pulse_spec
+  (t:G.erased trace)  //pulse_spec
+  (record:record_t)  //pulse_spec
+  (#rrepr:erased repr_t { trace_and_record_valid_for_derive_child t rrepr })  //pulse_spec
+  requires record_perm record 1.0R rrepr **  //pulse_spec
+           sid_pts_to trace_ref sid t  //pulse_spec
+  returns b:bool  //pulse_spec
+  ensures derive_child_client_perm sid t rrepr b  //pulse_spec
 {
-  intro_record_and_repr_tag_related record 1.0R rrepr;
+  intro_record_and_repr_tag_related record 1.0R rrepr;  //pulse_proof
 
-  rewrite emp as (session_state_related InUse (G_InUse (current_state t)));
-  let s = replace_session sid t InUse (G_InUse (current_state t));
-  with t1. assert (sid_pts_to trace_ref sid t1);
+  rewrite emp as (session_state_related InUse (G_InUse (current_state t)));  //pulse_proof
+  let s = replace_session sid t InUse (G_InUse (current_state t));  //pulse_code
+  with t1. assert (sid_pts_to trace_ref sid t1);  //pulse_proof
 
-  match s {
-    Available hc -> {
-      match hc.context {
-        L1_context _ -> {
-          rewrite (session_state_related s (current_state t)) as
-                  (pure False);
-          unreachable ()
+  match s {  //pulse_code
+    Available hc -> {  //pulse_code
+      match hc.context {  //pulse_code
+        L1_context _ -> {  //pulse_code
+          rewrite (session_state_related s (current_state t)) as  //pulse_proof
+                  (pure False);  //pulse_proof
+          unreachable ()  //pulse_proof
         }
-        _ -> {
-          assume_ (pure (~ (L1_context? hc.context)));
-          let repr = rewrite_session_state_related_available hc.context s t;
-          intro_context_and_repr_tag_related hc.context repr;
-          let ret = derive_child_from_context hc.context record #rrepr #repr ();
+        _ -> {  //pulse_code
+          assume_ (pure (~ (L1_context? hc.context)));  //pulse_proof
+          let repr = rewrite_session_state_related_available hc.context s t;  //pulse_proof
+          intro_context_and_repr_tag_related hc.context repr;  //pulse_proof
+          let ret = derive_child_from_context hc.context record #rrepr #repr ();  //pulse_code
 
-          match ret {
-            Some nctxt -> {
-              unfold (maybe_context_perm repr rrepr (Some nctxt));
-              with nrepr. assert (context_perm nctxt nrepr);
-              intro_context_and_repr_tag_related nctxt nrepr;
-              let s = Available { context = nctxt };
-              rewrite (context_perm nctxt nrepr) as
-                      (session_state_related s (G_Available nrepr));
-              let s = replace_session sid t1 s (G_Available nrepr);
-              intro_session_state_tag_related s (current_state t1);
-              fold (derive_child_client_perm sid t rrepr true);
-              with _x _y. rewrite (session_state_related _x _y) as emp;
-              true
+          match ret {  //pulse_code
+            Some nctxt -> {  //pulse_code
+              unfold (maybe_context_perm repr rrepr (Some nctxt));  //pulse_proof
+              with nrepr. assert (context_perm nctxt nrepr);  //pulse_proof
+              intro_context_and_repr_tag_related nctxt nrepr;  //pulse_proof
+              let s = Available { context = nctxt };  //pulse_code
+              rewrite (context_perm nctxt nrepr) as  //pulse_proof
+                      (session_state_related s (G_Available nrepr));  //pulse_proof
+              let s = replace_session sid t1 s (G_Available nrepr);  //pulse_code
+              intro_session_state_tag_related s (current_state t1);  //pulse_proof
+              fold (derive_child_client_perm sid t rrepr true);  //pulse_proof
+              with _x _y. rewrite (session_state_related _x _y) as emp;  //pulse_proof
+              true  //pulse_code
             }
-            None -> {
-              let s = SessionError;
-              rewrite (maybe_context_perm repr rrepr ret) as emp;
-              rewrite emp as (session_state_related s (G_SessionError (current_state t1)));
-              let s = replace_session sid t1 s (G_SessionError (current_state t1));
-              intro_session_state_tag_related s (current_state t1);
-              fold (derive_child_client_perm sid t rrepr false);
-              with _x _y. rewrite (session_state_related _x _y) as emp;
-              false
+            None -> {  //pulse_code
+              let s = SessionError;  //pulse_code
+              rewrite (maybe_context_perm repr rrepr ret) as emp;  //pulse_proof
+              rewrite emp as (session_state_related s (G_SessionError (current_state t1)));  //pulse_proof
+              let s = replace_session sid t1 s (G_SessionError (current_state t1));  //pulse_code
+              intro_session_state_tag_related s (current_state t1);  //pulse_proof
+              fold (derive_child_client_perm sid t rrepr false);  //pulse_proof
+              with _x _y. rewrite (session_state_related _x _y) as emp;  //pulse_proof
+              false  //pulse_code
             }
           }
         }
       }
     }
-    SessionStart -> {
-      rewrite (session_state_related s (current_state t)) as
-              (pure False);
-      unreachable ()
+    SessionStart -> {  //pulse_code
+      rewrite (session_state_related s (current_state t)) as  //pulse_proof
+              (pure False);  //pulse_proof
+      unreachable ()  //pulse_proof
     }
-    InUse -> {
-      rewrite (session_state_related s (current_state t)) as
-              (pure False);
-      unreachable ()
+    InUse -> {  //pulse_code
+      rewrite (session_state_related s (current_state t)) as  //pulse_proof
+              (pure False);  //pulse_proof
+      unreachable ()  //pulse_proof
     }
-    SessionClosed -> {
-      rewrite (session_state_related s (current_state t)) as
-              (pure False);
-      unreachable ()
+    SessionClosed -> {  //pulse_code
+      rewrite (session_state_related s (current_state t)) as  //pulse_proof
+              (pure False);  //pulse_proof
+      unreachable ()  //pulse_proof
     }
-    SessionError -> {
-      rewrite (session_state_related s (current_state t)) as
-              (pure False);
-      unreachable ()
-    }
-  }
-}
-```
-
-```pulse
-fn destroy_session_state (s:session_state) (t:G.erased trace)
-  requires session_state_related s (current_state t)
-  ensures emp
-{
-  intro_session_state_tag_related s (current_state t);
-  match s {
-    Available hc -> {
-      rewrite_session_state_related_available hc.context s t;
-      destroy_ctxt hc.context
-    }
-    _ -> {
-      assume_ (pure (~ (Available? s)));
-      with _x _y. rewrite (session_state_related _x _y) as emp
+    SessionError -> {  //pulse_code
+      rewrite (session_state_related s (current_state t)) as  //pulse_proof
+              (pure False);  //pulse_proof
+      unreachable ()  //pulse_proof
     }
   }
 }
 ```
 
 ```pulse
-fn close_session (sid:sid_t)
-  (t:G.erased trace { trace_valid_for_close t })
-  requires sid_pts_to trace_ref sid t
-  ensures session_closed_client_perm sid t
+fn destroy_session_state (s:session_state) (t:G.erased trace)  //pulse_spec
+  requires session_state_related s (current_state t)  //pulse_spec
+  ensures emp  //pulse_spec
 {
-  rewrite emp as (session_state_related InUse (G_InUse (current_state t)));
-  let s = replace_session sid t InUse (G_InUse (current_state t));
-  with t1. assert (sid_pts_to trace_ref sid t1);
+  intro_session_state_tag_related s (current_state t);  //pulse_proof
+  match s {  //pulse_code
+    Available hc -> {  //pulse_code
+      rewrite_session_state_related_available hc.context s t;  //pulse_proof
+      destroy_ctxt hc.context  //pulse_code
+    }
+    _ -> {  //pulse_code
+      assume_ (pure (~ (Available? s)));  //pulse_proof
+      with _x _y. rewrite (session_state_related _x _y) as emp  //pulse_proof
+    }
+  }
+}
+```
 
-  intro_session_state_tag_related s (current_state t);
+```pulse
+fn close_session (sid:sid_t)  //pulse_spec
+  (t:G.erased trace { trace_valid_for_close t })  //pulse_spec
+  requires sid_pts_to trace_ref sid t  //pulse_spec
+  ensures session_closed_client_perm sid t  //pulse_spec
+{
+  rewrite emp as (session_state_related InUse (G_InUse (current_state t)));  //pulse_proof
+  let s = replace_session sid t InUse (G_InUse (current_state t));  //pulse_code
+  with t1. assert (sid_pts_to trace_ref sid t1);  //pulse_proof
 
-  destroy_session_state s t;
+  intro_session_state_tag_related s (current_state t);  //pulse_proof
 
-  rewrite emp as (session_state_related SessionClosed (G_SessionClosed (current_state t1)));
-  let s = replace_session sid t1 SessionClosed (G_SessionClosed (current_state t1));
-  intro_session_state_tag_related s (current_state t1);
-  with _x _y. rewrite (session_state_related _x _y) as emp;
-  fold (session_closed_client_perm sid t)
+  destroy_session_state s t;  //pulse_code
+
+  rewrite emp as (session_state_related SessionClosed (G_SessionClosed (current_state t1)));  //pulse_proof
+  let s = replace_session sid t1 SessionClosed (G_SessionClosed (current_state t1));  //pulse_code
+  intro_session_state_tag_related s (current_state t1);  //pulse_proof
+  with _x _y. rewrite (session_state_related _x _y) as emp;  //pulse_proof
+  fold (session_closed_client_perm sid t)  //pulse_proof
 }
 ```
 
 #push-options "--z3rlimit_factor 4 --fuel 2 --ifuel 1 --split_queries no"
 ```pulse
-fn certify_key (sid:sid_t)
-  (pub_key:A.larray U8.t 32)
-  (crt_len:U32.t)
-  (crt:A.larray U8.t (U32.v crt_len))
-  (t:G.erased trace { trace_valid_for_certify_key t })
-  requires sid_pts_to trace_ref sid t **
-           (exists* pub_key_repr crt_repr.
-              A.pts_to pub_key pub_key_repr **
-              A.pts_to crt crt_repr)
-  returns _:U32.t
-  ensures certify_key_client_perm sid t **
-          (exists* pub_key_repr crt_repr.
-             A.pts_to pub_key pub_key_repr **
-             A.pts_to crt crt_repr)
+fn certify_key (sid:sid_t)  //pulse_spec
+  (pub_key:A.larray U8.t 32)  //pulse_spec
+  (crt_len:U32.t)  //pulse_spec
+  (crt:A.larray U8.t (U32.v crt_len))  //pulse_spec
+  (t:G.erased trace { trace_valid_for_certify_key t })  //pulse_spec
+  requires sid_pts_to trace_ref sid t **  //pulse_spec
+           (exists* pub_key_repr crt_repr.  //pulse_spec
+              A.pts_to pub_key pub_key_repr **  //pulse_spec
+              A.pts_to crt crt_repr)  //pulse_spec
+  returns _:U32.t  //pulse_spec
+  ensures certify_key_client_perm sid t **  //pulse_spec
+          (exists* pub_key_repr crt_repr.  //pulse_spec
+             A.pts_to pub_key pub_key_repr **  //pulse_spec
+             A.pts_to crt crt_repr)  //pulse_spec
 {
-  rewrite emp as (session_state_related InUse (G_InUse (current_state t)));
-  let s = replace_session sid t InUse (G_InUse (current_state t));
-  with t1. assert (sid_pts_to trace_ref sid t1);
+  rewrite emp as (session_state_related InUse (G_InUse (current_state t)));  //pulse_proof
+  let s = replace_session sid t InUse (G_InUse (current_state t));  //pulse_code
+  with t1. assert (sid_pts_to trace_ref sid t1);  //pulse_proof
 
-  match s {
-    Available hc -> {
-      match hc.context {
-        L1_context c -> {
-          let c_crt_len = c.aliasKeyCRT_len;
-          if U32.lt crt_len c_crt_len {
-            let ns = Available { context = L1_context c };
-            rewrite (session_state_related s (current_state t)) as
-                    (session_state_related ns (current_state t));
-            let s = replace_session sid t1 ns (current_state t);
-            intro_session_state_tag_related s (current_state t1);
-            with _x _y. rewrite (session_state_related _x _y) as emp;
-            fold (certify_key_client_perm sid t);
-            0ul
-          } else {
-            let r = rewrite_session_state_related_available (L1_context c) s t;
-            let r = rewrite_context_perm_l1 c;
-            unfold (l1_context_perm c r);
+  match s {  //pulse_code
+    Available hc -> {  //pulse_code
+      match hc.context {  //pulse_code
+        L1_context c -> {  //pulse_code
+          let c_crt_len = c.aliasKeyCRT_len;  //pulse_code
+          if U32.lt crt_len c_crt_len {  //pulse_code
+            let ns = Available { context = L1_context c };  //pulse_code
+            rewrite (session_state_related s (current_state t)) as  //pulse_proof
+                    (session_state_related ns (current_state t));  //pulse_proof
+            let s = replace_session sid t1 ns (current_state t);  //pulse_code
+            intro_session_state_tag_related s (current_state t1);  //pulse_proof
+            with _x _y. rewrite (session_state_related _x _y) as emp;  //pulse_proof
+            fold (certify_key_client_perm sid t);  //pulse_proof
+            0ul  //pulse_code
+          } else {  //pulse_code
+            let r = rewrite_session_state_related_available (L1_context c) s t;  //pulse_proof
+            let r = rewrite_context_perm_l1 c;  //pulse_proof
+            unfold (l1_context_perm c r);  //pulse_proof
 
-            V.to_array_pts_to c.aliasKey_pub;
-            memcpy_l (SZ.uint_to_t 32) (V.vec_to_array c.aliasKey_pub) pub_key;
-            V.to_vec_pts_to c.aliasKey_pub;
+            V.to_array_pts_to c.aliasKey_pub;  //pulse_proof
+            memcpy_l (SZ.uint_to_t 32) (V.vec_to_array c.aliasKey_pub) pub_key;  //pulse_code
+            V.to_vec_pts_to c.aliasKey_pub;  //pulse_proof
 
-            assume_ (pure (SZ.fits_u32));
-            V.to_array_pts_to c.aliasKeyCRT;
+            assume_ (pure (SZ.fits_u32));  //pulse_proof
+            V.to_array_pts_to c.aliasKeyCRT;  //pulse_proof
             
-            memcpy_l (SZ.uint32_to_sizet c.aliasKeyCRT_len) (V.vec_to_array c.aliasKeyCRT) crt;
-            V.to_vec_pts_to c.aliasKeyCRT;
+            memcpy_l (SZ.uint32_to_sizet c.aliasKeyCRT_len) (V.vec_to_array c.aliasKeyCRT) crt;  //pulse_code
+            V.to_vec_pts_to c.aliasKeyCRT;  //pulse_proof
 
-            fold (l1_context_perm c r);
-            rewrite (l1_context_perm c r) as
-                    (context_perm (L1_context c) (L1_context_repr r));
+            fold (l1_context_perm c r);  //pulse_proof
+            rewrite (l1_context_perm c r) as  //pulse_proof
+                    (context_perm (L1_context c) (L1_context_repr r));  //pulse_proof
             
-            let ns = Available { context = L1_context c };
-            rewrite (context_perm (L1_context c) (L1_context_repr r)) as
-                    (session_state_related ns (current_state t));
+            let ns = Available { context = L1_context c };  //pulse_code
+            rewrite (context_perm (L1_context c) (L1_context_repr r)) as  //pulse_proof
+                    (session_state_related ns (current_state t));  //pulse_proof
             
-            let s = replace_session sid t1 ns (current_state t);
-            intro_session_state_tag_related s (current_state t1);
-            with _x _y. rewrite (session_state_related _x _y) as emp;
-            fold (certify_key_client_perm sid t);
-            c_crt_len
+            let s = replace_session sid t1 ns (current_state t);  //pulse_code
+            intro_session_state_tag_related s (current_state t1);  //pulse_proof
+            with _x _y. rewrite (session_state_related _x _y) as emp;  //pulse_proof
+            fold (certify_key_client_perm sid t);  //pulse_proof
+            c_crt_len  //pulse_code
           }
         }
-        _ -> {
-          assume_ (pure (~ (L1_context? hc.context)));
-          rewrite (session_state_related s (current_state t)) as
-                  (pure False);
-          unreachable ()
+        _ -> {  //pulse_code
+          assume_ (pure (~ (L1_context? hc.context)));  //pulse_proof
+          rewrite (session_state_related s (current_state t)) as  //pulse_proof
+                  (pure False);  //pulse_proof
+          unreachable ()  //pulse_proof
         }
       }
     }
-    _ -> {
-      assume_ (pure (~ (Available? s)));
-      rewrite (session_state_related s (current_state t)) as
-              (pure False);
-      unreachable ()
+    _ -> {  //pulse_code
+      assume_ (pure (~ (Available? s)));  //pulse_proof
+      rewrite (session_state_related s (current_state t)) as  //pulse_proof
+              (pure False);  //pulse_proof
+      unreachable ()  //pulse_proof
     }
   }
 }
@@ -1308,62 +1308,62 @@ fn certify_key (sid:sid_t)
 
 #push-options "--split_queries no"
 ```pulse
-fn sign (sid:sid_t)
-  (signature:A.larray U8.t 64)
-  (msg_len:SZ.t { SZ.v msg_len < pow2 32 })
-  (msg:A.larray U8.t (SZ.v msg_len))
-  (t:G.erased trace { trace_valid_for_sign t })
-  requires sid_pts_to trace_ref sid t **
-           (exists* signature_repr msg_repr.
-              A.pts_to signature signature_repr **
-              A.pts_to msg msg_repr)
-  ensures sign_client_perm sid t **
-          (exists* signature_repr msg_repr.
-             A.pts_to signature signature_repr **
-             A.pts_to msg msg_repr)
+fn sign (sid:sid_t)  //pulse_spec
+  (signature:A.larray U8.t 64)  //pulse_spec
+  (msg_len:SZ.t { SZ.v msg_len < pow2 32 })  //pulse_spec
+  (msg:A.larray U8.t (SZ.v msg_len))  //pulse_spec
+  (t:G.erased trace { trace_valid_for_sign t })  //pulse_spec
+  requires sid_pts_to trace_ref sid t **  //pulse_spec
+           (exists* signature_repr msg_repr.  //pulse_spec
+              A.pts_to signature signature_repr **  //pulse_spec
+              A.pts_to msg msg_repr)  //pulse_spec
+  ensures sign_client_perm sid t **  //pulse_spec
+          (exists* signature_repr msg_repr.  //pulse_spec
+             A.pts_to signature signature_repr **  //pulse_spec
+             A.pts_to msg msg_repr)  //pulse_spec
 {
-  rewrite emp as (session_state_related InUse (G_InUse (current_state t)));
-  let s = replace_session sid t InUse (G_InUse (current_state t));
-  with t1. assert (sid_pts_to trace_ref sid t1);
+  rewrite emp as (session_state_related InUse (G_InUse (current_state t)));  //pulse_proof
+  let s = replace_session sid t InUse (G_InUse (current_state t));  //pulse_code
+  with t1. assert (sid_pts_to trace_ref sid t1);  //pulse_proof
 
-  match s {
-    Available hc -> {
-      match hc.context {
-        L1_context c -> {
-          let r = rewrite_session_state_related_available (L1_context c) s t;
-          let r = rewrite_context_perm_l1 c;
-          unfold (l1_context_perm c r);
+  match s {  //pulse_code
+    Available hc -> {  //pulse_code
+      match hc.context {  //pulse_code
+        L1_context c -> {  //pulse_code
+          let r = rewrite_session_state_related_available (L1_context c) s t;  //pulse_proof
+          let r = rewrite_context_perm_l1 c;  //pulse_proof
+          unfold (l1_context_perm c r);  //pulse_proof
 
-          V.to_array_pts_to c.aliasKey_priv;
-          HACL.ed25519_sign signature (V.vec_to_array c.aliasKey_priv) msg_len msg;
-          V.to_vec_pts_to c.aliasKey_priv;
+          V.to_array_pts_to c.aliasKey_priv;  //pulse_proof
+          HACL.ed25519_sign signature (V.vec_to_array c.aliasKey_priv) msg_len msg;  //pulse_code
+          V.to_vec_pts_to c.aliasKey_priv;  //pulse_proof
 
-          fold (l1_context_perm c r);
-          rewrite (l1_context_perm c r) as
-                  (context_perm (L1_context c) (L1_context_repr r));
+          fold (l1_context_perm c r);  //pulse_proof
+          rewrite (l1_context_perm c r) as  //pulse_proof
+                  (context_perm (L1_context c) (L1_context_repr r));  //pulse_proof
             
-          let ns = Available { context = L1_context c };
-          rewrite (context_perm (L1_context c) (L1_context_repr r)) as
-                  (session_state_related ns (current_state t));
+          let ns = Available { context = L1_context c };  //pulse_code
+          rewrite (context_perm (L1_context c) (L1_context_repr r)) as  //pulse_proof
+                  (session_state_related ns (current_state t));  //pulse_proof
             
-          let s = replace_session sid t1 ns (current_state t);
-          intro_session_state_tag_related s (current_state t1);
-          with _x _y. rewrite (session_state_related _x _y) as emp;
-          fold (sign_client_perm sid t);
+          let s = replace_session sid t1 ns (current_state t);  //pulse_code
+          intro_session_state_tag_related s (current_state t1);  //pulse_proof
+          with _x _y. rewrite (session_state_related _x _y) as emp;  //pulse_proof
+          fold (sign_client_perm sid t);  //pulse_proof
         }
-        _ -> {
-          assume_ (pure (~ (L1_context? hc.context)));
-          rewrite (session_state_related s (current_state t)) as
-                  (pure False);
-          unreachable ()
+        _ -> {  //pulse_code
+          assume_ (pure (~ (L1_context? hc.context)));  //pulse_proof
+          rewrite (session_state_related s (current_state t)) as  //pulse_proof
+                  (pure False);  //pulse_proof
+          unreachable ()  //pulse_proof
         }
       }
     }
-    _ -> {
-      assume_ (pure (~ (Available? s)));
-      rewrite (session_state_related s (current_state t)) as
-              (pure False);
-      unreachable ()
+    _ -> {  //pulse_code
+      assume_ (pure (~ (Available? s)));  //pulse_proof
+      rewrite (session_state_related s (current_state t)) as  //pulse_proof
+              (pure False);  //pulse_proof
+      unreachable ()  //pulse_proof
     }
   }
 }
